src/InferWidthsnew.v
@@ -1,0 +1,1822 @@
+From Coq Require Import FunInd FMaps FMapAVL OrderedType ZArith.
+From mathcomp Require Import ssreflect ssrbool ssrnat ssrint eqtype seq ssrfun.
+From simplssrlib Require Import Types SsrOrder FSets FMaps Tactics Var Store.
+From nbits Require Import NBits.
+From firrtl Require Import Firrtl Env HiEnv HiFirrtl ModuleGraph TopoSort. 
+
+Fixpoint tmap_type_size (t : ftype) : N :=
+(* calculates how many entries in tmap.env would be created/affected by a variable of type t *)
+match t with
+| Gtyp _ => 1
+| Atyp t _ => tmap_type_size t (* only one entry is needed for the array *)
+| Btyp ff => tmap_type_size_fields ff
+end
+with tmap_type_size_fields (ff : ffield) : N :=
+match ff with
+| Fnil => 0
+| Fflips _ _ ft ff' => tmap_type_size ft + tmap_type_size_fields ff'
+end.
+
+(* 以下函数都是只考虑gtyp的版本，并且array只考虑一个元素 *)
+Fixpoint ft_find_sub (checkt : ftype) (num : N) : option fgtyp :=
+  match checkt with
+  | Gtyp gt => if num == N0 then Some gt else None
+  | Atyp atyp n => ft_find_sub atyp num
+  | Btyp ff => if num >= (tmap_type_size_fields) ff then None else ft_find_ff ff num 
+  end
+with ft_find_ff (ff : ffield) (num : N) : option fgtyp :=
+  match ff with
+  | Fflips v0 _ ft ff' => if num >= (N.of_nat (tmap_type_size ft)) (* 不在该field中, 找下一个field *)
+                              then ft_find_ff ff' (N.sub num (N.of_nat (num_ref ft)))
+                           else (* 在field v0中 *)
+                              ft_find_sub ft num
+  | _ => None
+  end.
+
+Fixpoint ft_check_flip (checkt : ftype) (num : N) (fl : bool) : option bool :=
+  match checkt with
+  | Gtyp gt => if num == N0 then Some fl else None
+  | Atyp atyp n => ft_check_flip atyp num fl
+  | Btyp ff => if num >= (tmap_type_size_fields) ff then None else ft_check_flip_f ff num fl
+  end
+with ft_check_flip_f (ff : ffield) (num : N) (fl : bool) : option bool :=
+  match ff with
+  | Fflips v0 Flipped ft ff' => if num >= (N.of_nat (tmap_type_size ft)) (* 不在该field中, 找下一个field *)
+                                  then ft_check_flip_f ff' (N.sub num (N.of_nat (num_ref ft))) fl
+                              else (* 在field v0中 *)
+                                  ft_check_flip ft num (~~fl)
+  | Fflips v0 Nflip ft ff' => if num >= (N.of_nat (tmap_type_size ft)) (* 不在该field中, 找下一个field *)
+                                  then ft_check_flip_f ff' (N.sub num (N.of_nat (num_ref ft))) fl
+                              else (* 在field v0中 *)
+                                  ft_check_flip ft num fl
+  | _ => None
+  end.
+
+Fixpoint ft_set_sub (checkt : ftype) (newt : fgtyp) (num : N) : option ftype :=
+  match checkt with
+  | Gtyp _ => if num == N0 then Some (Gtyp newt) else None
+  | Atyp atyp n => match ft_set_sub atyp newt num with
+                      | Some natyp => Some (Atyp natyp n)
+                      | None => None
+                      end
+  | Btyp ff => if num >= (tmap_type_size_fields) ff then None else
+                match ft_set_sub_f ff newt num with
+                | Some newf => Some (Btyp newf)
+                | None => None
+                end
+  end
+with ft_set_sub_f (ff : ffield) (newt : fgtyp) (num : N) : option ffield :=
+  match ff with
+  | Fflips v0 fl ft ff' => if N.to_nat num >= (tmap_type_size ft) (* 不在该field中, 找下一个field *)
+                            then match ft_set_sub_f ff' newt (N.sub num (N.of_nat (tmap_type_size ft))) with
+                                | Some newf => Some (Fflips v0 fl ft newf)
+                                | None => None
+                                end
+                          else (* 在field v0中 *)
+                            match ft_set_sub ft newt num with
+                            | Some newt' => Some (Fflips v0 fl newt' ff')
+                            | None => None
+                            end
+  | _ => None
+  end.
+
+(* 有必要check这几个函数功能是否正确 *)
+Definition testaty0 := (Atyp (Gtyp (Fuint_implicit 0)) 2).
+Definition testaty := (Atyp (Atyp (Gtyp (Fuint 4)) 2) 2).
+Definition testbty0 := (Btyp (Fflips (1%num) Nflip (Atyp (Gtyp (Fuint_implicit 0)) 2) (Fflips (1%num) Nflip (Atyp (Gtyp (Fuint_implicit 1)) 2) Fnil))).
+Definition testbty := (Btyp (Fflips (1%num) Flipped (Btyp (Fflips (1%num) Nflip (Gtyp (Fuint_implicit 0)) (Fflips (1%num) Flipped (Atyp (Gtyp (Fuint_implicit 1)) 2) Fnil))) (Fflips (1%num) Nflip (Atyp (Gtyp (Fuint_implicit 2)) 2) Fnil))).
+Definition testgt := (Fuint 4).
+Compute (tmap_type_size testaty). 
+Compute (ft_find_sub testbty 2%num).
+Compute (ft_check_flip testbty 2%num false).
+Compute (ft_set_sub testbty testgt 3%num).
+
+Definition port_tmap (tmap : CEP.t ftype) (p : HiFP.hfport) : CEP.t ftype :=
+(* Extend a tmap with one port
+   tmap_expli: pair (tmap, names of fully-explicit ports)
+   p: port
+   output: a pair (tmap with the variables for p added, names of fully-explicit ports (possibly including p))
+   This function assumes implicitly that if there is a port identifier (v, n),
+   there is no other port with identifier (v, n') that clashes with it (i.e. the difference |n - n'|
+   is too small to accommodate the ground-type elements of one of them). *)
+match p with
+| Finput (v, n) t | Foutput (v, n) t =>
+    CEP.add (v, n) t tmap
+end.
+
+Definition ports_tmap (ps : seq HiFP.hfport) : CEP.t ftype :=
+(* create a tmap containing the variables for the ports in ps *)
+seq.foldl port_tmap (CEP.empty ftype) ps.
+
+(* type of mux expression *)
+Fixpoint mux_types (t1 : ftype) (t2 : ftype) : option ftype :=
+      match t1, t2 with
+      | Gtyp (Fuint w1), Gtyp (Fuint w2) => Some (Gtyp (Fuint (maxn w1 w2)))
+      | Gtyp (Fsint w1), Gtyp (Fsint w2) => Some (Gtyp (Fsint (maxn w1 w2)))
+      | Gtyp Fclock, Gtyp Fclock => Some (Gtyp Fclock)
+      | Gtyp Freset, Gtyp Freset => Some (Gtyp Freset)
+      | Gtyp Fasyncreset, Gtyp Fasyncreset => Some (Gtyp Fasyncreset)
+      | Atyp t1' n1, Atyp t2' n2 => match n1 == n2, mux_types t1' t2' with
+                                    | true, Some t => Some (Atyp t n1)
+                                    | _, _ => None
+                                    end
+      | Btyp bs1, Btyp bs2 =>
+          match mux_btyps bs1 bs2 with
+          | Some ff => Some (Btyp ff)
+          | None => None
+          end
+      | _, _ => None
+      end
+with mux_btyps (bs1 : ffield) (bs2 : ffield) : option ffield :=
+      match bs1, bs2 with
+      | Fnil, Fnil => Some Fnil
+      | Fflips v1 Nflip t1 fs1, Fflips v2 Nflip t2 fs2 =>
+          if v1 == v2 then match mux_types t1 t2, mux_btyps fs1 fs2 with
+                           | Some t, Some fs => Some (Fflips v1 Nflip t fs)
+                           | _, _ => None
+                           end
+                      else None
+      (* mux types must be passive, so Flipped is not allowed *)
+      | _, _ => None
+    end.
+
+Fixpoint base_ref_fields (base : VarOrder.t * N) (v : VarOrder.t) (ff : ffield) : option (VarOrder.t * N * ftype) :=
+(* find field v in ff. If found, return its type as an auxiliary to base_ref. *)
+match ff with
+| Fnil => None
+| Fflips v' _ t' ff' =>
+    if v == v' then Some (base, t')
+               else base_ref_fields (base.1, (base.2 + tmap_type_size t')%num) v ff'
+end.
+
+Fixpoint base_ref (ref : HiFP.href) (tmap : CEP.t ftype) : option (VarOrder.t * N * ftype) :=
+(* For reference ref, finds the pair (v, n) and the type that corresponds to it.
+(v,n) is the first item in the list of variables associated to ref that is affected by it.
+This function counts n for tmap, i.e. all arrays are treated as having only one element. *)
+match ref with
+| Eid v =>
+    match CEP.find v tmap with
+    | Some t => Some (v, t)
+    | None   => None
+    end
+| Esubfield ref' v' =>
+    match base_ref ref' tmap with
+    | Some (base, Btyp ff) => base_ref_fields base v' ff
+    | _ => None
+    end
+| Esubindex ref' _
+| Esubaccess ref' _ =>
+    match base_ref ref' tmap with
+    | Some (base, Atyp t' _) => Some (base, t')
+    | _ => None
+    end
+end.
+
+Fixpoint type_of_hfexpr (e : HiFP.hfexpr) (ce : CEP.t ftype) : option ftype :=
+(* calculates the type of the expression e.
+   In contrast to HiFP.type_of_hfexpr, this function only needs the map of types,
+   and it will preserve the information whether some ground type has an implicit width
+   (I am not sure yet whether that information needs to be preserved at all.)
+   Should the width of variables be preserved faithfully? Not sure at this moment;
+   perhaps we need two versions. *)
+match e with
+| Econst t _ => Some (Gtyp t)
+| Eref r => match base_ref r ce with
+            | Some (_, ft) => Some ft
+            | None => None
+            end
+| Ecast AsUInt e1 => match type_of_hfexpr e1 ce with
+                     | Some (Gtyp (Fsint w)) | Some (Gtyp (Fuint w)) => Some (Gtyp (Fuint w))
+                     | Some (Gtyp (Fsint_implicit w)) | Some (Gtyp (Fuint_implicit w)) => Some (Gtyp (Fuint_implicit w))
+                     | Some (Gtyp Fclock) | Some (Gtyp Freset) | Some (Gtyp Fasyncreset) => Some (Gtyp (Fuint 1))
+                     | _ => None
+                     end
+| Ecast AsSInt e1 => match type_of_hfexpr e1 ce with
+                     | Some (Gtyp (Fsint w)) | Some (Gtyp (Fuint w)) => Some (Gtyp (Fsint w))
+                     | Some (Gtyp (Fsint_implicit w)) | Some (Gtyp (Fuint_implicit w)) => Some (Gtyp (Fsint_implicit w))
+                     | Some (Gtyp Fclock) | Some (Gtyp Freset) | Some (Gtyp Fasyncreset) => Some (Gtyp (Fsint 1))
+                     | _ => None
+                     end
+| Ecast AsClock e1 => match type_of_hfexpr e1 ce with
+                      | Some (Gtyp _) => Some (Gtyp Fclock)
+                      | _ => None
+                      end
+| Ecast AsReset e1 => match type_of_hfexpr e1 ce with
+                      | Some (Gtyp _) => Some (Gtyp Freset)
+                      | _ => None
+                      end
+| Ecast AsAsync e1 => match type_of_hfexpr e1 ce  with
+                      | Some (Gtyp _) => Some (Gtyp Fasyncreset)
+                      | _ => None
+                      end
+| Eprim_unop (Upad n) e1 => match type_of_hfexpr e1 ce with
+                            | Some (Gtyp (Fsint w)) => Some (Gtyp (Fsint (maxn w n)))
+                            | Some (Gtyp (Fuint w)) => Some (Gtyp (Fuint (maxn w n)))
+                            | Some (Gtyp (Fsint_implicit w)) => Some (Gtyp (Fsint_implicit (maxn w n)))
+                            | Some (Gtyp (Fuint_implicit w)) => Some (Gtyp (Fuint_implicit (maxn w n)))
+                            | _ => None
+                            end
+| Eprim_unop (Ushl n) e1 => match type_of_hfexpr e1 ce with
+                            | Some (Gtyp (Fsint w)) => Some (Gtyp (Fsint (w + n)))
+                            | Some (Gtyp (Fuint w)) => Some (Gtyp (Fuint (w + n)))
+                            | Some (Gtyp (Fsint_implicit w)) => Some (Gtyp (Fsint_implicit (w + n)))
+                            | Some (Gtyp (Fuint_implicit w)) => Some (Gtyp (Fuint_implicit (w + n)))
+                            | _ => None
+                            end
+| Eprim_unop (Ushr n) e1 => match type_of_hfexpr e1 ce with
+                            | Some (Gtyp (Fsint w)) => Some (Gtyp (Fsint (maxn (w - n) 1)))
+                            | Some (Gtyp (Fuint w)) => Some (Gtyp (Fuint (maxn (w - n) 1)))
+                            | Some (Gtyp (Fsint_implicit w)) => Some (Gtyp (Fsint_implicit (maxn (w - n) 1)))
+                            | Some (Gtyp (Fuint_implicit w)) => Some (Gtyp (Fuint_implicit (maxn (w - n) 1)))
+                            | _ => None
+                            end
+| Eprim_unop Ucvt e1 => match type_of_hfexpr e1 ce with
+                        | Some (Gtyp (Fsint w)) => Some (Gtyp (Fsint w))
+                        | Some (Gtyp (Fuint w)) => Some (Gtyp (Fsint (w + 1)))
+                        | Some (Gtyp (Fsint_implicit w)) => Some (Gtyp (Fsint_implicit w))
+                        | Some (Gtyp (Fuint_implicit w)) => Some (Gtyp (Fsint_implicit (w + 1)))
+                        | _ => None
+                        end
+| Eprim_unop Uneg e1 => match type_of_hfexpr e1 ce with
+                        | Some (Gtyp (Fsint w)) | Some (Gtyp (Fuint w)) => Some (Gtyp (Fsint (w + 1)))
+                        | Some (Gtyp (Fsint_implicit w)) | Some (Gtyp (Fuint_implicit w)) => Some (Gtyp (Fsint_implicit (w + 1)))
+                        | _ => None
+                        end
+| Eprim_unop Unot e1 => match type_of_hfexpr e1 ce with
+                        | Some (Gtyp (Fsint w)) | Some (Gtyp (Fuint w)) => Some (Gtyp (Fuint w))
+                        | Some (Gtyp (Fsint_implicit w)) | Some (Gtyp (Fuint_implicit w)) => Some (Gtyp (Fuint_implicit w))
+                        | _ => None
+                        end
+| Eprim_unop (Uextr n1 n2) e1 => match type_of_hfexpr e1 ce with
+                                 | Some (Gtyp (Fsint w)) | Some (Gtyp (Fuint w))
+                                 | Some (Gtyp (Fsint_implicit w)) | Some (Gtyp (Fuint_implicit w)) =>
+                                      if (n2 <= n1) && (n1 < w) then Some (Gtyp (Fuint (n1 - n2 + 1)))
+                                                                else None
+                                 | _ => None
+                                 end
+| Eprim_unop (Uhead n) e1 => match type_of_hfexpr e1 ce with
+                             | Some (Gtyp (Fsint w)) | Some (Gtyp (Fuint w))
+                             | Some (Gtyp (Fsint_implicit w)) | Some (Gtyp (Fuint_implicit w)) =>
+                                 if n <= w then Some (Gtyp (Fuint n))
+                                           else None
+                             | _ => None
+                             end
+| Eprim_unop (Utail n) e1 => match type_of_hfexpr e1 ce with
+                             | Some (Gtyp (Fsint w)) | Some (Gtyp (Fuint w))
+                             | Some (Gtyp (Fsint_implicit w)) | Some (Gtyp (Fuint_implicit w)) =>
+                                 if n <= w then Some (Gtyp (Fuint (w - n)))
+                                           else None
+                             | _ => None
+                             end
+| Eprim_unop _ e1 => match type_of_hfexpr e1 ce with
+                     | Some (Gtyp (Fsint _)) | Some (Gtyp (Fuint _))
+                     | Some (Gtyp (Fsint_implicit _)) | Some (Gtyp (Fuint_implicit _)) => Some (Gtyp (Fuint 1))
+                     | _ => None
+                     end
+| Eprim_binop (Bcomp _) e1 e2 => match type_of_hfexpr e1 ce, type_of_hfexpr e2 ce with
+                                 | Some (Gtyp (Fsint _)), Some (Gtyp (Fsint _))
+                                 | Some (Gtyp (Fsint _)), Some (Gtyp (Fsint_implicit _))
+                                 | Some (Gtyp (Fsint_implicit _)), Some (Gtyp (Fsint _))
+                                 | Some (Gtyp (Fsint_implicit _)), Some (Gtyp (Fsint_implicit _))
+                                 | Some (Gtyp (Fuint _)), Some (Gtyp (Fuint _))
+                                 | Some (Gtyp (Fuint _)), Some (Gtyp (Fuint_implicit _))
+                                 | Some (Gtyp (Fuint_implicit _)), Some (Gtyp (Fuint _))
+                                 | Some (Gtyp (Fuint_implicit _)), Some (Gtyp (Fuint_implicit _)) =>
+                                     Some (Gtyp (Fuint 1))
+                                 | _, _ => None
+                                 end
+| Eprim_binop Badd e1 e2
+| Eprim_binop Bsub e1 e2 => match type_of_hfexpr e1 ce, type_of_hfexpr e2 ce with
+                            | Some (Gtyp (Fuint w1)), Some (Gtyp (Fuint w2)) => Some (Gtyp (Fuint (maxn w1 w2 + 1)))
+                            | Some (Gtyp (Fuint w1)), Some (Gtyp (Fuint_implicit w2))
+                            | Some (Gtyp (Fuint_implicit w1)), Some (Gtyp (Fuint w2))
+                            | Some (Gtyp (Fuint_implicit w1)), Some (Gtyp (Fuint_implicit w2)) =>
+                                Some (Gtyp (Fuint_implicit (maxn w1 w2 + 1)))
+                            | Some (Gtyp (Fsint w1)), Some (Gtyp (Fsint w2)) => Some (Gtyp (Fsint (maxn w1 w2 + 1)))
+                            | Some (Gtyp (Fsint w1)), Some (Gtyp (Fsint_implicit w2))
+                            | Some (Gtyp (Fsint_implicit w1)), Some (Gtyp (Fsint w2))
+                            | Some (Gtyp (Fsint_implicit w1)), Some (Gtyp (Fsint_implicit w2)) =>
+                                Some (Gtyp (Fsint_implicit (maxn w1 w2 + 1)))
+                            | _, _ => None
+                            end
+| Eprim_binop Bmul e1 e2 => match type_of_hfexpr e1 ce, type_of_hfexpr e2 ce with
+                            | Some (Gtyp (Fuint w1)), Some (Gtyp (Fuint w2)) => Some (Gtyp (Fuint (w1 + w2)))
+                            | Some (Gtyp (Fuint w1)), Some (Gtyp (Fuint_implicit w2))
+                            | Some (Gtyp (Fuint_implicit w1)), Some (Gtyp (Fuint w2))
+                            | Some (Gtyp (Fuint_implicit w1)), Some (Gtyp (Fuint_implicit w2)) =>
+                                Some (Gtyp (Fuint_implicit (w1 + w2)))
+                            | Some (Gtyp (Fsint w1)), Some (Gtyp (Fsint w2)) => Some (Gtyp (Fsint (w1 + w2)))
+                            | Some (Gtyp (Fsint w1)), Some (Gtyp (Fsint_implicit w2))
+                            | Some (Gtyp (Fsint_implicit w1)), Some (Gtyp (Fsint w2))
+                            | Some (Gtyp (Fsint_implicit w1)), Some (Gtyp (Fsint_implicit w2)) =>
+                                Some (Gtyp (Fsint_implicit (w1 + w2)))
+                            | _, _ => None
+                            end
+| Eprim_binop Bdiv e1 e2  => match type_of_hfexpr e1 ce, type_of_hfexpr e2 ce with
+                             | Some (Gtyp (Fuint w1)), Some (Gtyp (Fuint _))
+                             | Some (Gtyp (Fuint w1)), Some (Gtyp (Fuint_implicit _)) => Some (Gtyp (Fuint w1))
+                             | Some (Gtyp (Fuint_implicit w1)), Some (Gtyp (Fuint _))
+                             | Some (Gtyp (Fuint_implicit w1)), Some (Gtyp (Fuint_implicit _)) => Some (Gtyp (Fuint_implicit w1))
+                             | Some (Gtyp (Fsint w1)), Some (Gtyp (Fsint _))
+                             | Some (Gtyp (Fsint w1)), Some (Gtyp (Fsint_implicit _)) => Some (Gtyp (Fsint (w1 + 1)))
+                             | Some (Gtyp (Fsint_implicit w1)), Some (Gtyp (Fsint _))
+                             | Some (Gtyp (Fsint_implicit w1)), Some (Gtyp (Fsint_implicit _)) => Some (Gtyp (Fsint_implicit (w1 + 1)))
+                             | _, _ => None
+                             end
+| Eprim_binop Brem e1 e2 => match type_of_hfexpr e1 ce, type_of_hfexpr e2 ce with
+                            | Some (Gtyp (Fuint w1)), Some (Gtyp (Fuint w2)) => Some (Gtyp (Fuint (minn w1 w2)))
+                            | Some (Gtyp (Fuint w1)), Some (Gtyp (Fuint_implicit w2))
+                            | Some (Gtyp (Fuint_implicit w1)), Some (Gtyp (Fuint w2))
+                            | Some (Gtyp (Fuint_implicit w1)), Some (Gtyp (Fuint_implicit w2)) =>
+                                Some (Gtyp (Fuint_implicit (minn w1 w2)))
+                            | Some (Gtyp (Fsint w1)), Some (Gtyp (Fsint w2)) => Some (Gtyp (Fsint (minn w1 w2)))
+                            | Some (Gtyp (Fsint w1)), Some (Gtyp (Fsint_implicit w2))
+                            | Some (Gtyp (Fsint_implicit w1)), Some (Gtyp (Fsint w2))
+                            | Some (Gtyp (Fsint_implicit w1)), Some (Gtyp (Fsint_implicit w2)) =>
+                                Some (Gtyp (Fsint_implicit (minn w1 w2)))
+                            | _, _ => None
+                            end
+| Eprim_binop Bdshl e1 e2 => match type_of_hfexpr e1 ce, type_of_hfexpr e2 ce with
+                             | Some (Gtyp (Fuint w1)), Some (Gtyp (Fuint w2)) => Some (Gtyp (Fuint (w1 + 2 ^ w2 - 1)))
+                             | Some (Gtyp (Fuint w1)), Some (Gtyp (Fuint_implicit w2))
+                             | Some (Gtyp (Fuint_implicit w1)), Some (Gtyp (Fuint w2))
+                             | Some (Gtyp (Fuint_implicit w1)), Some (Gtyp (Fuint_implicit w2)) => Some (Gtyp (Fuint_implicit (w1 + 2 ^ w2 - 1)))
+                             | Some (Gtyp (Fsint w1)), Some (Gtyp (Fuint w2)) => Some (Gtyp (Fsint (w1 + 2 ^ w2 - 1)))
+                             | Some (Gtyp (Fsint w1)), Some (Gtyp (Fsint_implicit w2))
+                             | Some (Gtyp (Fsint_implicit w1)), Some (Gtyp (Fsint w2))
+                             | Some (Gtyp (Fsint_implicit w1)), Some (Gtyp (Fsint_implicit w2)) => Some (Gtyp (Fsint_implicit (w1 + 2 ^ w2 - 1)))
+                             | _, _ => None
+                             end
+| Eprim_binop Bdshr e1 e2 => match type_of_hfexpr e1 ce, type_of_hfexpr e2 ce with
+                             | Some (Gtyp (Fuint w1)), Some (Gtyp (Fuint _))
+                             | Some (Gtyp (Fuint w1)), Some (Gtyp (Fuint_implicit _)) => Some (Gtyp (Fuint w1))
+                             | Some (Gtyp (Fuint_implicit w1)), Some (Gtyp (Fuint _))
+                             | Some (Gtyp (Fuint_implicit w1)), Some (Gtyp (Fuint_implicit _)) => Some (Gtyp (Fuint_implicit w1))
+                             | Some (Gtyp (Fsint w1)), Some (Gtyp (Fuint _))
+                             | Some (Gtyp (Fsint w1)), Some (Gtyp (Fuint_implicit _)) => Some (Gtyp (Fsint w1))
+                             | Some (Gtyp (Fsint_implicit w1)), Some (Gtyp (Fuint _))
+                             | Some (Gtyp (Fsint_implicit w1)), Some (Gtyp (Fuint_implicit _)) => Some (Gtyp (Fsint_implicit w1))
+                             | _, _ => None
+                             end
+| Eprim_binop Bcat e1 e2 => match type_of_hfexpr e1 ce, type_of_hfexpr e2 ce with
+                            | Some (Gtyp (Fuint w1)), Some (Gtyp (Fuint w2))
+                            | Some (Gtyp (Fsint w1)), Some (Gtyp (Fsint w2)) => Some (Gtyp (Fuint (w1 + w2)))
+                            | Some (Gtyp (Fuint w1)), Some (Gtyp (Fuint_implicit w2))
+                            | Some (Gtyp (Fuint_implicit w1)), Some (Gtyp (Fuint w2))
+                            | Some (Gtyp (Fuint_implicit w1)), Some (Gtyp (Fuint_implicit w2))
+                            | Some (Gtyp (Fsint w1)), Some (Gtyp (Fsint_implicit w2))
+                            | Some (Gtyp (Fsint_implicit w1)), Some (Gtyp (Fsint w2))
+                            | Some (Gtyp (Fsint_implicit w1)), Some (Gtyp (Fsint_implicit w2)) =>
+                                Some (Gtyp (Fuint_implicit (w1 + w2)))
+                            | _, _ => None
+                            end
+| Eprim_binop Band e1 e2
+| Eprim_binop Bor e1 e2
+| Eprim_binop Bxor e1 e2 => match type_of_hfexpr e1 ce, type_of_hfexpr e2 ce with
+                            | Some (Gtyp (Fuint w1)), Some (Gtyp (Fuint w2))
+                            | Some (Gtyp (Fuint w1)), Some (Gtyp (Fuint_implicit w2))
+                            | Some (Gtyp (Fuint_implicit w1)), Some (Gtyp (Fuint w2))
+                            | Some (Gtyp (Fuint_implicit w1)), Some (Gtyp (Fuint_implicit w2))
+                            | Some (Gtyp (Fsint w1)), Some (Gtyp (Fsint w2))
+                            | Some (Gtyp (Fsint w1)), Some (Gtyp (Fsint_implicit w2))
+                            | Some (Gtyp (Fsint_implicit w1)), Some (Gtyp (Fsint w2))
+                            | Some (Gtyp (Fsint_implicit w1)), Some (Gtyp (Fsint_implicit w2)) => Some (Gtyp (Fuint (maxn w1 w2)))
+                            | _, _ => None
+                            end
+| Emux c e1 e2 => match type_of_hfexpr c ce, type_of_hfexpr e1 ce, type_of_hfexpr e2 ce with
+                  | Some (Gtyp (Fuint 1)), Some t1, Some t2
+                  | Some (Gtyp (Fuint_implicit 1)), Some t1, Some t2 =>
+                      mux_types t1 t2
+                  | _, _, _ => None
+                  end
+| Evalidif c e1 => match type_of_hfexpr c ce with
+                   | Some (Gtyp (Fuint 1)) | Some (Gtyp (Fuint_implicit 1)) => type_of_hfexpr e1 ce
+                   | _ => None
+                   end
+end.
+
+Fixpoint tmap_add_bidir_connect (m_nt_ns : var2exprsmap * N * N) (v_tgt : VarOrder.t) (ref_tgt : HiFP.href) (t_tgt : ftype) (v_src : VarOrder.t) (ref_src : HiFP.href) (t_src : ftype) : option (var2exprsmap * N * N) :=
+(* check whether types are compatible and add connections for all ground-type entries of ref_tgt <= ref_src,
+   while taking into account flipped fields.
+   This works for InferWidths, so for arrays it only adds one connection, not one connection per entry.
+   m_n is a pair: a var2exprsmap to which connections are added
+                  a natural number that indicates which index of ref_tgt and ref_src is to be connected
+   v_tgt and v_src are variable names.
+   ref_tgt and ref_src are the respective hrefs that correspond to (v_tgt, m_nt_ns.1.2) and (v_src, m_nt_ns.2).
+   The return value is a triple where the first element is the updated var2exprsmap and
+   the second and third is increased by as many connections as there have been added. *)
+match t_tgt, t_src with
+| Gtyp (Fuint _), Gtyp (Fuint _) | Gtyp (Fuint _), Gtyp (Fuint_implicit _)
+| Gtyp (Fsint _), Gtyp (Fsint _) | Gtyp (Fsint _), Gtyp (Fsint_implicit _)
+| Gtyp Fclock, Gtyp Fclock
+| Gtyp Freset, Gtyp Freset
+| Gtyp Fasyncreset, Gtyp Fasyncreset =>
+    (* the target has explicit width, do not register the connection *)
+    Some (m_nt_ns.1.1, (m_nt_ns.1.2 + 1)%num, (m_nt_ns.2 + 1)%num)
+| Gtyp (Fuint_implicit _), Gtyp (Fuint _) | Gtyp (Fuint_implicit _), Gtyp (Fuint_implicit _)
+| Gtyp (Fsint_implicit _), Gtyp (Fsint _) | Gtyp (Fsint_implicit _), Gtyp (Fsint_implicit _) =>
+    Some (match module_graph_vertex_set_p.find (v_tgt, m_nt_ns.1.2) m_nt_ns.1.1 with
+          | Some expr_list => module_graph_vertex_set_p.add (v_tgt, m_nt_ns.1.2)    (Eref ref_src :: expr_list) m_nt_ns.1.1
+          | None =>           module_graph_vertex_set_p.add (v_tgt, m_nt_ns.1.2) [:: Eref ref_src]              m_nt_ns.1.1
+          end, (m_nt_ns.1.2 + 1)%num, (m_nt_ns.2 + 1)%num)
+| Atyp t_tgt' n_tgt, Atyp t_src' n_src =>
+    if n_tgt != n_src then None
+    else tmap_add_bidir_connect m_nt_ns v_tgt (Esubindex ref_tgt 0) t_tgt' v_src (Esubindex ref_src 0) t_src'
+| Btyp ff_tgt, Btyp ff_src => tmap_add_bidir_connect_fields m_nt_ns v_tgt ref_tgt ff_tgt v_src ref_src ff_src
+| _, _ => None
+end
+with tmap_add_bidir_connect_fields (m_nt_ns : var2exprsmap * N * N) (v_tgt : VarOrder.t) (ref_tgt : HiFP.href) (ff_tgt : ffield) (v_src : VarOrder.t) (ref_src : HiFP.href) (ff_src : ffield) : option (var2exprsmap * N * N) :=
+(* check whether types are compatible and add connections for all ground-type entries of ref_tgt <= ref_src,
+   where these are bundle types with types (Btyp ff_tgt) and (Btyp ff_src), respectively. *)
+match ff_tgt, ff_src with
+| Fnil, Fnil => Some m_nt_ns
+| Fflips v_tgt Nflip t_tgt ff_tgt', Fflips v_src Nflip t_src ff_src' =>
+    if v_tgt != v_src then None
+    else if tmap_add_bidir_connect m_nt_ns v_tgt (Esubfield ref_tgt v_tgt) t_tgt v_src (Esubfield ref_src v_src) t_src is Some m_nt_ns'
+         then tmap_add_bidir_connect_fields m_nt_ns' v_tgt ref_tgt ff_tgt' v_src ref_src ff_src'
+         else None
+| Fflips v_tgt Flipped t_tgt ff_tgt', Fflips v_src Flipped t_src ff_src' =>
+    if v_tgt != v_src then None
+    else if tmap_add_bidir_connect_flipped m_nt_ns v_tgt (Esubfield ref_tgt v_tgt) t_tgt v_src (Esubfield ref_src v_src) t_src is Some m_nt_ns'
+         then tmap_add_bidir_connect_fields m_nt_ns' v_tgt ref_tgt ff_tgt' v_src ref_src ff_src'
+         else None
+| _, _ => None
+end
+with tmap_add_bidir_connect_flipped (m_nt_ns : var2exprsmap * N * N) (v_tgt : VarOrder.t) (ref_tgt : HiFP.href) (t_tgt : ftype) (v_src : VarOrder.t) (ref_src : HiFP.href) (t_src : ftype) : option (var2exprsmap * N * N) :=
+(* check whether types are compatible and add connections for all ground-type entries of ref_src <= ref_tgt,
+   i.e. the other direction than tmap_add_bidir_connect. *)
+match t_tgt, t_src with
+| Gtyp (Fuint _), Gtyp (Fuint _) | Gtyp (Fuint_implicit _), Gtyp (Fuint _)
+| Gtyp (Fsint _), Gtyp (Fsint _) | Gtyp (Fsint_implicit _), Gtyp (Fsint _)
+| Gtyp Fclock, Gtyp Fclock
+| Gtyp Freset, Gtyp Freset
+| Gtyp Fasyncreset, Gtyp Fasyncreset =>
+    (* the target has explicit width, do not register the connection *)
+    Some (m_nt_ns.1.1, (m_nt_ns.1.2 + 1)%num, (m_nt_ns.2 + 1)%num)
+| Gtyp (Fuint _), Gtyp (Fuint_implicit _) | Gtyp (Fuint_implicit _), Gtyp (Fuint_implicit _)
+| Gtyp (Fsint _), Gtyp (Fsint_implicit _) | Gtyp (Fsint_implicit _), Gtyp (Fsint_implicit _) =>
+    Some (match module_graph_vertex_set_p.find (v_src, m_nt_ns.2) m_nt_ns.1.1 with
+          | Some expr_list => module_graph_vertex_set_p.add (v_src, m_nt_ns.2)    (Eref ref_tgt :: expr_list) m_nt_ns.1.1
+          | None =>           module_graph_vertex_set_p.add (v_src, m_nt_ns.2) [:: Eref ref_tgt]              m_nt_ns.1.1
+          end, (m_nt_ns.1.2 + 1)%num, (m_nt_ns.2 + 1)%num)
+| Atyp t_tgt' n_tgt, Atyp t_src' n_src =>
+    if n_tgt != n_src then None
+    else tmap_add_bidir_connect_flipped m_nt_ns v_tgt (Esubindex ref_tgt 0) t_tgt' v_src (Esubindex ref_src 0) t_src'
+| Btyp ff_tgt, Btyp ff_src => tmap_add_bidir_connect_flipped_fields m_nt_ns v_tgt ref_tgt ff_tgt v_src ref_src ff_src
+| _, _ => None
+end
+with tmap_add_bidir_connect_flipped_fields (m_nt_ns : var2exprsmap * N * N) (v_tgt : VarOrder.t) (ref_tgt : HiFP.href) (ff_tgt : ffield) (v_src : VarOrder.t) (ref_src : HiFP.href) (ff_src : ffield) : option (var2exprsmap * N * N) :=
+(* check whether types are compatible and add connections for all ground-type entries of ref_src <= ref_tgt,
+   where these are bundle types with types (Btyp ff_src) and (Btyp ff_tgt), respectively,
+   i.e. the other direction than tmap_add_bidir_connect_fields. *)
+match ff_tgt, ff_src with
+| Fnil, Fnil => Some m_nt_ns
+| Fflips v_tgt Nflip t_tgt ff_tgt', Fflips v_src Nflip t_src ff_src' =>
+    if v_tgt != v_src then None
+    else if tmap_add_bidir_connect_flipped m_nt_ns v_tgt (Esubfield ref_tgt v_tgt) t_tgt v_src (Esubfield ref_src v_src) t_src is Some m_nt_ns'
+         then tmap_add_bidir_connect_flipped_fields m_nt_ns' v_tgt ref_tgt ff_tgt' v_src ref_src ff_src'
+         else None
+| Fflips v_tgt Flipped t_tgt ff_tgt', Fflips v_src Flipped t_src ff_src' =>
+    if v_tgt != v_src then None
+    else if tmap_add_bidir_connect m_nt_ns v_tgt (Esubfield ref_tgt v_tgt) t_tgt v_src (Esubfield ref_src v_src) t_src is Some m_nt_ns'
+         then tmap_add_bidir_connect_flipped_fields m_nt_ns' v_tgt ref_tgt ff_tgt' v_src ref_src ff_src'
+         else None
+| _, _ => None
+end.
+
+Fixpoint tmap_add_passive_connect (m_nt : var2exprsmap * N) (v_tgt : VarOrder.t) (ref_src : HiFP.href) (t : ftype) : option (var2exprsmap * N) :=
+(* passive version of tmap_add_bidir_connect.
+   This works for InferWidths, so for arrays it only adds one connection, not one connection per entry.
+   m_nt is a pair: a var2exprsmap to which connections are added
+                  a natural number that indicates which index of ref_tgt and ref_src is to be connected
+   v_tgt is the variable name.
+   ref_src is the href that v_tgt is connected to.
+   The return value is a pair where the first element is the updated var2exprsmap and
+   the second element is increased by as many connections as there have been added. *)
+match t with
+| Gtyp (Fuint_implicit _)
+| Gtyp (Fsint_implicit _) =>
+    match module_graph_vertex_set_p.find (v_tgt, m_nt.2) m_nt.1 with
+    | Some expr_list => Some (module_graph_vertex_set_p.add (v_tgt, m_nt.2)    (Eref ref_src :: expr_list) m_nt.1, (m_nt.2 + 1)%num)
+    | None =>           Some (module_graph_vertex_set_p.add (v_tgt, m_nt.2) [:: Eref ref_src]              m_nt.1, (m_nt.2 + 1)%num)
+    end
+| Gtyp _ => Some (m_nt.1, (m_nt.2 + 1)%num)
+| Atyp t' _ => tmap_add_passive_connect m_nt v_tgt (Esubindex ref_src 0) t'
+| Btyp ff => tmap_add_passive_connect_fields m_nt v_tgt ref_src ff
+end
+with tmap_add_passive_connect_fields (m_nt : var2exprsmap * N) (v_tgt : VarOrder.t) (ref_src : HiFP.href) (ff : ffield) : option (var2exprsmap * N) :=
+match ff with
+| Fnil => Some m_nt
+| Fflips v Nflip   t ff' =>
+    match tmap_add_passive_connect m_nt v_tgt (Esubfield ref_src v) t with
+    | Some m_nt' => tmap_add_passive_connect_fields m_nt' v_tgt ref_src ff'
+    | None => None
+    end
+| Fflips v Flipped t ff' => None
+end.
+
+Fixpoint split_expr (ref_src : HiFP.href) (t : ftype) : option (seq HiFP.href) :=
+  match t with
+  | Gtyp _ => Some [:: ref_src]
+  | Atyp atyp _ => split_expr (Esubindex ref_src 0) atyp
+  | Btyp ff => split_expr_f ref_src ff 
+  end
+with split_expr_f (ref_src : HiFP.href) (ff : ffield) : option (seq HiFP.href) :=
+  match ff with
+  | Fnil => Some nil
+  | Fflips v Nflip t ff' =>
+    match split_expr_f ref_src ff', split_expr (Esubfield ref_src v) t with
+    | Some ls, Some ls' => Some (ls' ++ ls)
+    | _,_ => None
+    end
+  | Fflips v Flipped t ff' => None
+  end.
+
+Fixpoint split_expr_non_passive (ref_src : HiFP.href) (t : ftype) (fl : bool) : option (seq (HiFP.href * bool)) :=
+  match t with
+  | Gtyp _ => Some [:: (ref_src, fl)]
+  | Atyp atyp _ => split_expr_non_passive (Esubindex ref_src 0) atyp fl
+  | Btyp ff => split_expr_non_passive_f ref_src ff fl
+  end
+with split_expr_non_passive_f (ref_src : HiFP.href) (ff : ffield) (fl : bool) : option (seq (HiFP.href * bool)) :=
+  match ff with
+  | Fnil => Some nil
+  | Fflips v Nflip t ff' =>
+    match split_expr_non_passive_f ref_src ff' fl, split_expr_non_passive (Esubfield ref_src v) t fl with
+    | Some ls, Some ls' => Some (ls' ++ ls)
+    | _,_ => None
+    end
+  | Fflips v Flipped t ff' => 
+    match split_expr_non_passive_f ref_src ff' (~~fl), split_expr_non_passive (Esubfield ref_src v) t (~~fl) with
+    | Some ls, Some ls' => Some (ls' ++ ls)
+    | _,_ => None
+    end
+  end.
+
+Fixpoint tmap_add_expr_connect (m_nt : var2exprsmap * N) (v_tgt : VarOrder.t) (expr_src : HiFP.hfexpr) (t : ftype) : option var2exprsmap :=
+(* add connections for all ground-type entries of ref_tgt <= expr_src.
+   This works for InferWidths, so for arrays it only adds one connection, not one connection per entry.
+   m_n is a pair: a var2exprsmap to which connections are added
+                  a natural number that indicates which index of ref_tgt is to be connected
+   v_tgt is the base variable name.
+   ref_tgt is the href that corresponds to (v_tgt, m_nt.2).
+   The return value is the updated var2exprsmap. *)
+match t, expr_src with
+| Gtyp (Fuint_implicit _), expr
+| Gtyp (Fsint_implicit _), expr =>
+    match module_graph_vertex_set_p.find (v_tgt, m_nt.2) m_nt.1 with
+    | Some expr_list => Some (module_graph_vertex_set_p.add (v_tgt, m_nt.2)    (expr_src :: expr_list) m_nt.1)
+    | None =>           Some (module_graph_vertex_set_p.add (v_tgt, m_nt.2) [:: expr_src]              m_nt.1)
+    end
+| Gtyp _, _ => Some m_nt.1
+(* In Emux and Evalidif (below) the condition is not important for width inference. So ignore it. *)
+| t, Emux _ e1 e2 =>
+    match tmap_add_expr_connect m_nt v_tgt e1 t with
+    | Some m' => tmap_add_expr_connect (m', m_nt.2) v_tgt e2 t
+    | None => None
+    end
+| t, Evalidif _ e => tmap_add_expr_connect m_nt v_tgt e t
+| t, Eref ref =>
+    match tmap_add_passive_connect m_nt v_tgt ref t with
+    | Some (m', _) => Some m'
+    | None => None
+    end
+| _, _ => None
+end.
+
+Fixpoint combine_mux_expr (c : HiFP.hfexpr) (el1 el2 : seq HiFP.hfexpr) : option (seq HiFP.hfexpr) :=
+  match el1, el2 with
+  | nil, nil => Some nil
+  | hd1 :: tl1, hd2 :: tl2 => match combine_mux_expr c tl1 tl2 with
+                            | Some muxl => Some ((Emux c hd1 hd2) :: muxl)
+                            | None => None
+                            end
+  | _, _ => None
+  end.
+
+Fixpoint split_expr_connect (expr_src : HiFP.hfexpr) (t : ftype) : option (seq HiFP.hfexpr) :=
+  match expr_src with
+  | Eref ref => match split_expr ref t with
+                | Some refl => Some (map (fun tref => (Eref tref)) refl)
+                | None => None
+                end
+  | Emux c e1 e2 => match split_expr_connect e1 t, split_expr_connect e2 t with
+                  | Some el1, Some el2 => combine_mux_expr c el1 el2
+                  | _ ,_ => None
+                  end
+  | _ => Some [:: expr_src] 
+  end.
+
+Definition connect_fgtyp_compatible (t_tgt t_src : fgtyp) : bool :=
+  if (not_implicit t_tgt) then true
+  else (sizeof_fgtyp t_tgt >= sizeof_fgtyp t_src) && fgtyp_equiv t_tgt t_src.
+
+Fixpoint check_connect_fgtyp_compatible (t_tgt t_src : ftype) (n : nat) : bool :=
+  match n with
+  | 0 => true
+  | S m => match ft_find_sub t_tgt (N.of_nat m), ft_find_sub t_src (N.of_nat m) with
+          | Some gt_tgt, Some gt_src => connect_fgtyp_compatible gt_tgt gt_src && check_connect_fgtyp_compatible t_tgt t_src m
+          | _,_ => false
+          end
+  end.
+
+Fixpoint check_connect_non_passive_fgtyp (t_tgt t_src : ftype) (n : nat) : bool :=
+  match n with
+  | 0 => true
+  | S m => match ft_check_flip t_tgt (N.of_nat m) false, ft_find_sub t_tgt (N.of_nat m), ft_find_sub t_src (N.of_nat m) with
+          | Some false, Some gt_tgt, Some gt_src => connect_fgtyp_compatible gt_tgt gt_src && check_connect_non_passive_fgtyp t_tgt t_src m
+          | Some true, Some gt_tgt, Some gt_src => connect_fgtyp_compatible gt_src gt_tgt && check_connect_non_passive_fgtyp t_tgt t_src m
+          | _,_,_ => false
+          end
+  end.
+
+Definition connect_non_passive_type (t_tgt : ftype) (t_src : ftype) : Prop :=
+  ftype_equiv t_tgt t_src && check_connect_non_passive_fgtyp t_tgt t_src (tmap_type_size t_tgt).
+
+Definition connect_type_compatible (t_tgt t_src : ftype) : bool :=
+  ftype_equiv t_tgt t_src && check_connect_fgtyp_compatible t_tgt t_src (tmap_type_size t_tgt).
+
+(*match list_gtyp t_tgt, list_gtyp t_src with
+  | nil, nil => true
+  | hd1 :: tl1, 
+match t_tgt, t_src with
+| Gtyp (Fuint _), Gtyp (Fuint _)
+| Gtyp (Fuint _), Gtyp (Fuint_implicit _)
+| Gtyp (Fuint_implicit _), Gtyp (Fuint _)
+| Gtyp (Fuint_implicit _), Gtyp (Fuint_implicit _)
+| Gtyp (Fsint _), Gtyp (Fsint _)
+| Gtyp (Fsint _), Gtyp (Fsint_implicit _)
+| Gtyp (Fsint_implicit _), Gtyp (Fsint _)
+| Gtyp (Fsint_implicit _), Gtyp (Fsint_implicit _)
+| Gtyp Fclock, Gtyp Fclock
+| Gtyp Freset, Gtyp Freset
+| Gtyp Fasyncreset, Gtyp Fasyncreset => true
+| Atyp t_tgt' n_tgt, Atyp t_src' n_src => (n_tgt == n_src) && connect_type_compatible t_tgt' t_src'
+| Btyp ff_tgt, Btyp ff_src => connect_type_compatible_fields ff_tgt ff_src
+| _, _ => false
+end
+with connect_type_compatible_fields (ff_tgt ff_src : ffield) : bool :=
+match ff_tgt, ff_src with
+| Fnil, Fnil => true
+| Fflips v_tgt f_tgt t_tgt ff_tgt', Fflips v_src f_src t_src ff_src' =>
+    (v_tgt == v_src) && (fflip_eqn f_tgt f_src) && connect_type_compatible t_tgt t_src && connect_type_compatible_fields ff_tgt' ff_src'
+| _, _ => false
+end. (* should be none flip *)
+*)
+
+Fixpoint add_expr_connect (v : ProdVarOrder.t) (el : seq HiFP.hfexpr) (var2exprs : var2exprsmap) : var2exprsmap :=
+  match el with
+  | nil => var2exprs
+  | hd :: tl => match module_graph_vertex_set_p.find v var2exprs with
+                | Some ls => add_expr_connect (v.1, N.add v.2 1%num) tl (module_graph_vertex_set_p.add v (hd :: ls) var2exprs)
+                | None => add_expr_connect (v.1, N.add v.2 1%num) tl (module_graph_vertex_set_p.add v [::hd] var2exprs)
+                end
+  end.
+
+Fixpoint add_expr_connect_non_passive (v_lhs v_rhs : ProdVarOrder.t) (el1 el2 : seq (HiFP.href * bool)) (var2exprs : var2exprsmap) : option var2exprsmap :=
+  match el1, el2 with
+  | nil, nil => Some var2exprs
+  | (ref1, false) :: tl1, (ref2, false) :: tl2 => 
+                match module_graph_vertex_set_p.find v_lhs var2exprs with
+                | Some ls => add_expr_connect_non_passive (v_lhs.1, N.add v_lhs.2 1%num) (v_rhs.1, N.add v_rhs.2 1%num) tl1 tl2 (module_graph_vertex_set_p.add v_lhs ((Eref ref1) :: ls) var2exprs)
+                | None => add_expr_connect_non_passive (v_lhs.1, N.add v_lhs.2 1%num) (v_rhs.1, N.add v_rhs.2 1%num) tl1 tl2 (module_graph_vertex_set_p.add v_lhs [::(Eref ref1)] var2exprs)
+                end
+  | (ref1, true) :: tl1, (ref2, true) :: tl2 => 
+                match module_graph_vertex_set_p.find v_rhs var2exprs with
+                | Some ls => add_expr_connect_non_passive (v_lhs.1, N.add v_lhs.2 1%num) (v_rhs.1, N.add v_rhs.2 1%num) tl1 tl2 (module_graph_vertex_set_p.add v_rhs ((Eref ref2) :: ls) var2exprs)
+                | None => add_expr_connect_non_passive (v_lhs.1, N.add v_lhs.2 1%num) (v_rhs.1, N.add v_rhs.2 1%num) tl1 tl2 (module_graph_vertex_set_p.add v_rhs [::(Eref ref2)] var2exprs)
+                end
+  | _, _ => None
+  end.
+
+Fixpoint stmt_tmap (t_v : CEP.t ftype * var2exprsmap) (s: HiFP.hfstmt) : option (CEP.t ftype * var2exprsmap) :=
+(* t_v is a pair: tmap of components defined before statement s;
+                  map that indicates all expressions assigned to a certain ground-type part of a component.
+   s is a statement.
+   the result is the pair t_v expanded with the information from s *)
+match s with
+| Sskip => Some t_v
+| Swire v t => if CEP.find v t_v.1 is None
+               then Some (CEP.add v t t_v.1, t_v.2)
+               else None
+| Sreg v r => match CEP.find v t_v.1, reset r with
+              | Some _, _ => None
+              | None, Rst _ rst_val => match split_expr_connect rst_val (type r) with
+                                      | Some rstl => Some (CEP.add v (type r) t_v.1, add_expr_connect v rstl t_v.2)
+                                      | None => None
+                                      end
+              | None, NRst => Some (CEP.add v (type r) t_v.1, t_v.2)
+              end
+| Smem v m => (* TBD *) None
+| Sinst v inst => (* TBD *) None
+| Snode v e =>
+    match CEP.find v t_v.1, type_of_hfexpr e t_v.1 with
+    | None, Some t => match split_expr_connect e t with
+                    | Some rstl => Some (CEP.add v t t_v.1, add_expr_connect v rstl t_v.2)
+                    | None => None
+                    end
+    | _, _ => None
+    end
+| Sfcnct ref_tgt (Eref ref_src) =>
+    match base_ref ref_tgt t_v.1, base_ref ref_src t_v.1 with
+    | Some (v_tgt, t_tgt), Some (v_src, t_src) =>
+      match split_expr_non_passive ref_tgt t_tgt false, split_expr_non_passive ref_src t_src false with
+      | Some lhsl, Some rhsl => match add_expr_connect_non_passive v_tgt v_src lhsl rhsl t_v.2 with
+                                | Some newv2e => Some (t_v.1, newv2e)
+                                | None => None
+                                end
+      | _, _ => None
+      end
+    | _, _ => None
+    end
+| Sfcnct ref_tgt expr_src =>
+    match base_ref ref_tgt t_v.1, type_of_hfexpr expr_src t_v.1 with
+    | Some (v, t_tgt), Some t_src =>
+        if connect_type_compatible t_tgt t_src
+          then match split_expr_connect expr_src t_src with
+          | Some rstl => Some (t_v.1, add_expr_connect v rstl t_v.2)
+          | None => None
+          end
+        else None
+    | _,_ => None
+    end
+| Sinvalid _ => Some t_v
+| Swhen c ss_t ss_f =>
+    match stmts_tmap t_v ss_t with
+    | Some t_v' => stmts_tmap t_v' ss_f
+    | None => None
+    end
+end
+with stmts_tmap (t_v : CEP.t ftype * var2exprsmap) (ss: HiFP.hfstmt_seq) : option (CEP.t ftype * var2exprsmap) :=
+match ss with
+| Qnil => Some t_v
+| Qcons s ss' =>
+    match stmt_tmap t_v s with
+    | Some t_v' => stmts_tmap t_v' ss'
+    | None => None
+    end
+end.
+
+(* Correctness theorem for stmts_tmap:
+- All of the below holds if the output is Some (tmap, var2exprsmap).
+  - The tmap contains exactly the entries for all components that appear in the statement sequence
+    (in addition to the input parameter). [“contains at least” is needed for correctness; “contains
+    at most” is only needed to show minimality.]
+  - The var2exprsmap contains all connections to implicit-width components declared in the statement sequence.
+  * The var2exprsmap does not contain any connection that is not present in the statement sequence
+    (if the input parameter var2exprsmap is the empty map).
+    [This is only needed to show minimality.] *)
+
+Fixpoint stmt_tmap_is_correct (t_in : CEP.t ftype) (v2e_in : var2exprsmap) (s : HiFP.hfstmt) (t_out: CEP.t ftype) (v2e_out: var2exprsmap) : Prop :=
+   match s with
+   | Swire v t => CEP.find v t_in = None ->
+                        CEP.find v t_out = Some t
+                     /\ (forall v' : ProdVarOrder.t, v != v' -> CEP.find v' t_in = CEP.find v' t_out)
+                     /\ module_graph_vertex_set_p.Equal v2e_in v2e_out
+   | Sreg v r => CEP.find v t_in = None ->
+                       CEP.find v t_out = Some (type r)
+                    /\ (forall v' : ProdVarOrder.t, v != v' -> CEP.find v' t_in = CEP.find v' t_out)
+                    /\ (reset r = NRst ProdVarOrder.T -> module_graph_vertex_set_p.Equal v2e_in v2e_out)
+   | Snode v e => CEP.find v t_in = None ->
+                  (type_of_hfexpr e t_in != None) ->
+                       CEP.find v t_out = type_of_hfexpr e t_in
+                    /\ (forall v' : ProdVarOrder.t, v != v' -> CEP.find v' t_in = CEP.find v' t_out)
+                    /\ (module_graph_vertex_set_p.Equal v2e_in v2e_out)
+   | Sfcnct v e =>    CEP.Equal t_in t_out
+                   /\ (* forall t : ftype, CEP.find v t_in = Some t -> the connection is in v2e*) True
+   | Swhen c ss_t ss_f => exists (t_internal : CEP.t ftype) (v2e_internal : var2exprsmap),
+                                stmts_tmap_is_correct t_in v2e_in ss_t t_internal v2e_internal
+                             /\ stmts_tmap_is_correct t_internal v2e_internal ss_f t_out v2e_out
+   | _ =>    CEP.Equal t_in t_out
+          /\ module_graph_vertex_set_p.Equal v2e_in v2e_out
+   end
+with stmts_tmap_is_correct (t_in : CEP.t ftype) (v2e_in : var2exprsmap) (ss : HiFP.hfstmt_seq) (t_out: CEP.t ftype) (v2e_out: var2exprsmap) : Prop :=
+   match ss with
+   | Qnil => CEP.Equal t_in t_out /\ module_graph_vertex_set_p.Equal v2e_in v2e_out
+   | Qcons s ss' => exists (t_internal : CEP.t ftype) (v2e_internal : var2exprsmap),
+                          stmt_tmap_is_correct t_in v2e_in s t_internal v2e_internal
+                       /\ stmts_tmap_is_correct t_internal v2e_internal ss' t_out v2e_out
+   end.
+
+Theorem stmts_tmap_correct :
+   forall (ss : HiFP.hfstmt_seq) (t_in : CEP.t ftype) (v2e_in: var2exprsmap) (t_out: CEP.t ftype) (v2e_out: var2exprsmap),
+      stmts_tmap (t_in, v2e_in) ss = Some (t_out, v2e_out) ->
+         stmts_tmap_is_correct t_in v2e_in ss t_out v2e_out.
+Proof.
+induction ss as [|s ss'].
+* intros.
+  simpl stmts_tmap_is_correct.
+  simpl stmts_tmap in H.
+  injection H ; intros.
+  split.
+  + unfold CEP.Equal ; intro ; rewrite H1 ; reflexivity.
+  + unfold module_graph_vertex_set_p.Equal ; intro ; rewrite H0 ; reflexivity.
+* intros.
+  simpl stmts_tmap_is_correct.
+  simpl stmts_tmap in H.
+  destruct (stmt_tmap (t_in, v2e_in) s) eqn: H0.
+  + destruct p as [t_internal v2e_internal].
+    exists t_internal, v2e_internal.
+    split.
+    - destruct s.
+      * (* Sskip *)
+        simpl stmt_tmap_is_correct.
+        simpl stmt_tmap in H0.
+        injection H0 ; intros.
+        split.
+        + intro ; rewrite H2 ; reflexivity.
+        + unfold module_graph_vertex_set_p.Equal ; intro ; rewrite H1 ; reflexivity.
+      * (* Swire *)
+        simpl stmt_tmap_is_correct.
+        simpl stmt_tmap in H0.
+        intro.
+        rewrite H1 in H0.
+        injection H0 ; intros.
+        split.
+        + rewrite -H3 CEP.Lemmas.find_add_eq // /HiFirrtl.PVM.SE.eq eq_refl //.
+        split.
+        + intros.
+          apply negbTE in H4.
+          rewrite -H3 CEP.Lemmas.find_add_neq // /HiFirrtl.PVM.SE.eq eq_sym H4 //.
+        + unfold module_graph_vertex_set_p.Equal ; intro ; rewrite H2 ; reflexivity.
+      * (* Sreg *)
+        simpl stmt_tmap_is_correct.
+        simpl stmt_tmap in H0.
+        intro.
+        rewrite H1 in H0.
+        destruct (reset h).
+        + injection H0 ; intros.
+          split.
+          - rewrite -H3 CEP.Lemmas.find_add_eq // /HiFirrtl.PVM.SE.eq eq_refl //.
+          split.
+          - intros.
+            apply negbTE in H4.
+            rewrite -H3 CEP.Lemmas.find_add_neq // /HiFirrtl.PVM.SE.eq eq_sym H4 //.
+          - unfold module_graph_vertex_set_p.Equal ; intro ; rewrite H2 ; reflexivity.
+        + destruct (tmap_add_expr_connect (v2e_in, s.2) s.1 h1 (type h)) eqn: Htmap ; rewrite Htmap in H0 ; try done.
+          injection H0 ; intros.
+          split.
+          - rewrite -H3 CEP.Lemmas.find_add_eq // /HiFirrtl.PVM.SE.eq eq_refl //.
+          - split ; try done.
+            intros.
+            apply negbTE in H4.
+            rewrite -H3 CEP.Lemmas.find_add_neq // /HiFirrtl.PVM.SE.eq eq_sym H4 //.
+      * (* Smem has not yet been implemented *)
+        unfold stmt_tmap in H0 ; done.
+      * (* Sinst has not yet been implemented *)
+        unfold stmt_tmap in H0 ; done.
+      * (* Snode *)
+        simpl stmt_tmap_is_correct.
+        simpl stmt_tmap in H0.
+        destruct (CEP.find s t_in) eqn: H1 ; try done.
+        destruct (type_of_hfexpr h t_in) eqn: H2 ; try done.
+        destruct (tmap_add_expr_connect (v2e_in, s.2) s.1 h f) eqn: H3 ; try done ; rewrite H3 in H0.
+        injection H0 ; intros.
+        split.
+        + intro.
+
+    - apply IHss ; exact H.
+  + discriminate H.
+Admitted.
+
+(* return a fgtyp with the larger width for gtyp *)
+Definition max_fgtyp (ft1 : fgtyp) (ft2 : fgtyp) : option fgtyp :=
+  match ft1, ft2 with
+  | Fuint w1, Fuint_implicit w2 => Some (Fuint_implicit (max w1 w2))
+  | Fsint w1, Fsint_implicit w2 => Some (Fsint_implicit (max w1 w2))
+  | Fuint_implicit w1, Fuint_implicit w2 => Some (Fuint_implicit (max w1 w2))
+  | Fsint_implicit w1, Fsint_implicit w2 => Some (Fsint_implicit (max w1 w2))
+  | _,_ => None
+  end.
+  
+Fixpoint expr2varlist (expr : HiFP.hfexpr) (tmap : CEP.t ftype) : option (seq ProdVarOrder.t) :=
+   (* Prepends to ls the list of variable/component identifiers accessed by the expression expr.
+      tmap is used to look up the identifiers.
+      DNJ: I think parameter ls is superfluous, it seems to be never used.  It could be replaced by [::]. *)
+   match expr with
+   | Econst _ _ => Some nil
+   | Eref ref => match base_ref ref tmap with
+                | Some (pv,_) => Some [:: pv]
+                | None => None
+                end
+  | Eprim_unop _ e1 => expr2varlist e1 tmap
+  | Eprim_binop _ e1 e2 => match expr2varlist e1 tmap, expr2varlist e2 tmap with
+                          | Some ls', Some ls'' => Some (ls' ++ ls'')
+                          | _,_ => None
+                          end
+  | Emux e1 e2 e3 => match expr2varlist e1 tmap, expr2varlist e2 tmap, expr2varlist e3 tmap with
+                    | Some ls', Some ls'', Some ls''' => Some (ls' ++ ls'' ++ ls''')
+                    | _,_,_ => None
+                    end
+  | Evalidif e1 e2 => match expr2varlist e1 tmap, expr2varlist e2 tmap with
+                      | Some ls', Some ls'' => Some (ls' ++ ls'')
+                      | _,_ => None
+                      end
+  | Ecast _ e => expr2varlist e tmap
+   end.
+
+Definition updg (key : ProdVarOrder.t) (v : seq ProdVarOrder.t) (map : ProdVarOrder.t -> seq ProdVarOrder.t) : ProdVarOrder.t -> seq ProdVarOrder.t :=
+    fun (y : ProdVarOrder.t) => if y == key then v else map y.
+
+Fixpoint drawel (v : ProdVarOrder.t) (el : seq HiFP.hfexpr) (tmap : CEP.t ftype) (newg : ProdVarOrder.t -> seq ProdVarOrder.t) (vertices : seq ProdVarOrder.t) : option ((ProdVarOrder.t -> seq ProdVarOrder.t) * (seq ProdVarOrder.t)) :=
+   (* recursively draw dependencies in el for element v *)
+   (* v: vertex in the dependency graph that is updated
+      el: list of expressions that need to be considered for adding dependency edges
+      tmap: map of (known) types of components
+      newg: current edges in the dependency graph
+      vertices: current vertices in the dependency graph
+      Return value: a pair (edges in the dependency graph, vertices in the dependency graph)
+      containing additionally the dependencies from el *)
+   match el with
+   | nil => Some (newg, vertices)
+   | e :: etl => let vl := expr2varlist e tmap in
+                 match vl with (* all elements appearing in e *)
+                 | Some ls => let g' := List.fold_left (fun tempg tempv => updg tempv (cons v (tempg tempv)) tempg) ls newg in
+                              drawel v etl tmap g' (vertices ++ ls)
+                 | None => None
+                 end
+   end.
+
+Fixpoint drawg depandencyls (tmap : CEP.t ftype) (expli_reg : seq ProdVarOrder.t) (newg : ProdVarOrder.t -> seq ProdVarOrder.t) (vertices : seq ProdVarOrder.t) : option ((ProdVarOrder.t -> seq ProdVarOrder.t) * (seq ProdVarOrder.t)) :=
+   (* construct the dependency graph:
+      depandencyls: list of pairs (vertex in the module graph, list of expressions)
+      tmap: map of (known) types of components
+      expli_reg: list of completely explicit-width components; they can be ignored
+      newg: current edges in the dependency graph (will be extended by drawel)
+      vertices: current vertices in the dependency graph (will be extended by drawel)
+      Return value: a pair (edges in the dependency graph, vertices in the dependency graph)
+      *)
+   match depandencyls with
+   (* list of all pairs (element as key, its connections as value) *)
+   | nil => Some (newg, vertices)
+  | (v, el) :: vtl => if ((fst v, N0) \in expli_reg) then drawg vtl tmap expli_reg newg vertices
+                      else match drawel v el tmap newg vertices with (* for a certain element v, draw dependencies in the el to newg *)
+                      | Some (g', vertices') => drawg vtl tmap expli_reg g' vertices'
+                      | None => None
+                      end
+  end.
+
+(* init 应该是implicit，l中无所谓 *)
+Fixpoint max_ftlist (l : seq fgtyp) (init : fgtyp): option fgtyp :=
+  match l with
+  | nil => Some init
+  | t :: tl => match max_ftlist tl init with
+              | Some t' => max_fgtyp t t'
+              | None => None
+              end
+  end.
+  
+Fixpoint fil_ftlist (l : seq (option ftype)) : option (seq fgtyp) :=
+  match l with
+  | nil => Some [::]
+  | (Some (Gtyp gt)) :: tl => match fil_ftlist tl with
+                      | Some tl' => Some (gt :: tl')
+                      | None => None
+                      end
+  | _ :: tl => None
+  end.
+
+Definition InferWidth_fun (v : ProdVarOrder.t) (el : seq HiFP.hfexpr) (tmap : CEP.t ftype) : option (CEP.t ftype) :=
+(* updates the width of v in tmap so that it is at least the width of the expressions in list el. *)
+  match fil_ftlist (map (fun e => type_of_hfexpr e tmap) el) with
+  | Some eftl => match CEP.find (fst v, N0) tmap with
+                | Some init => match ft_find_sub init v.2 with
+                                | Some initt => if not_implicit initt then Some tmap
+                                                       else match max_ftlist eftl initt with
+                                                        | Some nt => match ft_set_sub init nt v.2 with
+                                                                    | Some nt0 => Some (CEP.add (fst v, N0) nt0 tmap)
+                                                                    | None => None
+                                                                    end
+                                                        | None => None
+                                                        end
+                                | _ => None
+                                end
+                | None => None
+                end
+  | None => None
+  end.
+  
+Fixpoint InferWidths_fun (od : seq ProdVarOrder.t) (var2exprs : var2exprsmap) (tmap : CEP.t ftype) : option (CEP.t ftype) :=
+(* od contains the (implicit-width) ground-type subcomponents in topological order.
+   (It is ok if od contains other components, but it is not necessary.)
+   var2exprs is a map that maps every ground-type subcomponent to a list of expressions (namely expressions that the (sub)component is connected from).
+   tmap is the map of types for every component that has been defined (but there are no separate entries for subcomponents);
+   the result is a modified tmap, which ensures that the width of every implicit-width component is large enough. *)
+  match od with
+  | nil => Some tmap
+  | vhd :: vtl => match module_graph_vertex_set_p.find vhd var2exprs with 
+                  | Some el => match InferWidth_fun vhd el tmap with
+                          | Some tm => InferWidths_fun vtl var2exprs tm
+                          | None => None
+                          end
+                  | None => None
+                  end
+  end.
+
+Fixpoint list_expligref (n : nat) (pv : ProdVarOrder.t) (checkt : ftype) : option (seq ProdVarOrder.t) := 
+  match n with
+  | 0 => Some nil
+  | S m => match list_expligref m pv checkt, ft_find_sub checkt (N.of_nat m) with
+          | Some ls, Some gt => if not_implicit gt then Some ls
+                                else Some ((fst pv, N.add (snd pv) (N.of_nat m)) :: ls)
+          | _, _ => None
+          end
+  end.
+
+Fixpoint explireg_stmt (st : HiFP.hfstmt) : option (seq ProdVarOrder.t) :=
+  match st with
+  | Sskip => Some nil 
+  | Swire v t => Some nil
+  | Sreg v r => let len := tmap_type_size (type r) in 
+                list_expligref len v (type r)
+  | Smem v m => (*TBD*) Some nil
+  | Sinst v inst => (*TBD*) Some nil
+  | Snode v e => Some nil
+  | Sfcnct v e => Some nil
+  | Sinvalid _ => Some nil
+  | Swhen _ s1 s2 => match explireg_stmts s1 , explireg_stmts s2 with
+                    | Some ls, Some ls' => Some (ls ++ ls')
+                    | _,_ => None
+                    end
+  end
+with explireg_stmts (sts : HiFP.hfstmt_seq) :=
+  match sts with
+  | Qnil => Some nil
+  | Qcons s ss => match explireg_stmt s, explireg_stmts ss with
+                  | Some ls, Some ls' => Some (ls ++ ls')
+                  | _,_ => None
+                  end
+  end.
+
+Definition emptyg : (ProdVarOrder.t -> seq ProdVarOrder.t) := (fun _ => [::]).
+
+Definition InferWidths_stage1 (F : HiFP.hfmodule) : option (CEP.t ftype) :=
+(* infer widths of implicit-width components among the ports and statements in F.
+   A full version would not work on one module alone but on all modules in a circuit together,
+   but the principle remains the same. Therefore, let’s just run the algorithm on a single module for now. *)
+match F with
+| FExmod _ _ _ => None
+| FInmod v ps ss =>
+    match stmts_tmap (ports_tmap ps, module_graph_vertex_set_p.empty (seq HiFP.hfexpr)) ss, explireg_stmts ss with
+    | Some (tmap', var2exprs), Some expli_reg => (* tmap' : all the expli/uninferred impli aggr&gtyp are stored here
+                                            var2exprs : every connected elements are stored *)
+           match drawg (module_graph_vertex_set_p.elements var2exprs) tmap' expli_reg emptyg nil with
+           | Some (theg, vertices) => (* theg : new drawn graph
+                                         vertices : set for topo sort to start with *)
+               match TopoSort.topo_sort vertices theg with
+               | TopoSort.Sorted inferorder => InferWidths_fun inferorder var2exprs tmap'
+               | _ => None
+               end
+           | None => None
+           end
+       | _,_ => None
+       end
+end.
+
+Fixpoint expli_ftype (t : ftype) : ftype :=
+  match t with
+  | Gtyp (Fuint_implicit w) => Gtyp (Fuint w)
+  | Gtyp (Fsint_implicit w) => Gtyp (Fsint w)
+  | Gtyp _ => t
+  | Atyp t_ref n_ref => Atyp (expli_ftype t_ref) n_ref
+  | Btyp ff_ref => Btyp (expli_ftype_ff ff_ref)
+  end
+with expli_ftype_ff (ff_ref : ffield) : ffield :=
+  match ff_ref with
+  | Fflips v_ref Nflip t_ref ff_ref' => Fflips v_ref Nflip (expli_ftype t_ref) (expli_ftype_ff ff_ref') 
+  | Fflips v_ref Flipped t_ref ff_ref' => Fflips v_ref Flipped (expli_ftype t_ref) (expli_ftype_ff ff_ref') 
+  | Fnil => Fnil
+  end.
+
+Definition InferWidths_transp (p : HiFP.hfport) (tmap : CEP.t ftype) : option HiFP.hfport :=
+  (* changes the type in one port declaration, depending on the information in tmap, to an explicit-width type *)
+  match p with
+  | Finput v t => if (ftype_not_implicit t) then Some p
+                  else (match CEP.find v tmap with
+                  | Some ft => (* if t has implicit width, update the hfport with ft and change it to explicit width *)
+                                Some (Finput v (expli_ftype ft))
+                  | _ => None
+                  end)
+  | Foutput v t => if (ftype_not_implicit t) then Some p
+                  else (match CEP.find v tmap with
+                  | Some ft => (* if t has implicit width, update the hfport with ft and change it to explicit width *)
+                                Some (Foutput v (expli_ftype ft))
+                  | _ => None
+                  end)
+  end.
+
+Fixpoint InferWidths_transps (ps : seq HiFP.hfport) (tmap : CEP.t ftype) : option (seq HiFP.hfport) :=
+  (* changes the types in a sequence of port declarations, depending on the information in tmap, to explicit-width types *)
+  match ps with
+  | nil => Some nil
+  | p :: tl => match InferWidths_transp p tmap, InferWidths_transps tl tmap with
+                  | Some n, Some nss => Some (n :: nss)
+                  | _, _ => None
+                  end
+  end.
+
+Fixpoint InferWidths_transs (s : HiFP.hfstmt) (tmap : CEP.t ftype) : option HiFP.hfstmt :=
+(* with infered tmap, transform the ports and declarations *)
+  match s with
+  | Sskip => Some s
+  | Swire v t => if (ftype_not_implicit t) then Some s
+                  else (match CEP.find v tmap with
+                  | Some ft => (* if t has implicit width, update the hfstmt with ft and change it to explicit width *)
+                                Some (Swire v (expli_ftype ft))
+                  | _ => None
+                  end)
+  | Sreg v r => if (ftype_not_implicit (type r)) then Some s
+                else (match CEP.find v tmap with
+                | Some ft => (* if t has implicit width, update the hfstmt with ft and change it to explicit width *)
+                              Some (Sreg v (mk_freg (expli_ftype ft) (clock r) (reset r)))
+                | _ => None
+                end)
+  | Smem v m => (*TBD*) Some s
+  | Sinst v inst => (*TBD*) Some s
+  | Snode v e => Some s
+  | Sfcnct v e => Some s
+  | Sinvalid _ => Some s
+  | Swhen c s1 s2 => match InferWidths_transss s1 tmap, InferWidths_transss s2 tmap with
+                    | Some n1, Some n2 => Some (Swhen c n1 n2)
+                    | _, _ => None
+                    end
+  end
+with InferWidths_transss (sts : HiFP.hfstmt_seq) (tmap : CEP.t ftype) : option HiFP.hfstmt_seq :=
+  match sts with
+  | Qnil => Some (Qnil ProdVarOrder.T)
+  | Qcons s ss => match InferWidths_transs s tmap, InferWidths_transss ss tmap with
+                  | Some n, Some nss => Some (Qcons n nss)
+                  | _, _ => None
+                  end
+  end.
+
+Definition InferWidths_stage2 (F : HiFP.hfmodule) (tmap : CEP.t ftype) : option HiFP.hfmodule :=
+match F with
+  | FExmod _ _ _ => None
+  | FInmod v ps ss => match InferWidths_transps ps tmap, InferWidths_transss ss tmap with
+                      | Some nps, Some nss => Some (FInmod v nps nss)
+                      | _, _ => None
+                      end
+  end.
+
+(*Definition connect_non_passive_gt (gt_tgt : fgtyp) (gt_src : fgtyp) : Prop :=
+  match gt_tgt, gt_src with
+      | Fuint _, Fuint _
+      | Fuint _, Fuint_implicit _
+      | Fsint _, Fsint _
+      | Fsint _, Fsint_implicit _
+      | Fclock, Fclock
+      | Freset, Freset
+      | Fasyncreset, Fasyncreset => True
+      | Fuint_implicit wt, Fuint ws
+      | Fuint_implicit wt, Fuint_implicit ws
+      | Fsint_implicit wt, Fsint ws
+      | Fsint_implicit wt, Fsint_implicit ws => wt >= ws
+      | _, _ => False
+      end.
+
+Fixpoint connect_non_passive_type (ft_tgt : ftype) (ft_src : ftype) : Prop :=
+  match ft_tgt, ft_src with
+   | Gtyp gt_tgt, Gtyp gt_src => connect_non_passive_gt gt_tgt gt_src
+   | Atyp elt_tgt n1, Atyp elt_src n2 => n1 = n2 /\ connect_non_passive_type elt_tgt elt_src
+   | Btyp ft, Btyp fs => connect_non_passive_type_fields ft fs 
+   | _, _ => False
+   end
+with connect_non_passive_type_fields (ft_tgt : ffield) (ft_src : ffield) : Prop :=
+  match ft_tgt, ft_src with
+   | Fnil, Fnil => True
+   | Fflips v1 Nflip gtt ft, Fflips v2 Nflip gts fs => v1 = v2 /\
+         connect_non_passive_type gtt gts /\
+         connect_non_passive_type_fields ft fs 
+   | Fflips v1 Flipped gtt ft, Fflips v2 Flipped gts fs => v1 = v2 /\
+         connect_non_passive_type_flipped gts gtt /\
+         connect_non_passive_type_fields ft fs
+   | _, _ => False
+   end
+with connect_non_passive_type_flipped (ft_tgt : ftype) (ft_src : ftype) : Prop :=
+   (* The code in this predicate is the same as in connect_non_passive. *)
+   match ft_tgt, ft_src with
+   | Gtyp gt_tgt, Gtyp gt_src => connect_non_passive_gt gt_tgt gt_src
+   | Atyp elt_tgt n1, Atyp elt_src n2 => n1 = n2 /\ connect_non_passive_type_flipped elt_tgt elt_src
+   | Btyp ft, Btyp fs => connect_non_passive_type_fields_flipped ft fs 
+   | _, _ => False
+   end
+with connect_non_passive_type_fields_flipped (ft_tgt : ffield) (ft_src : ffield) : Prop :=
+   (* The code in this predicate is the same as in connect_non_passive_fields. *)
+   match ft_tgt, ft_src with
+   | Fnil, Fnil => True
+   | Fflips v1 Nflip gtt ft, Fflips v2 Nflip gts fs => v1 = v2 /\
+         connect_non_passive_type_flipped gtt gts /\
+         connect_non_passive_type_fields_flipped ft fs 
+   | Fflips v1 Flipped gtt ft, Fflips v2 Flipped gts fs => v1 = v2 /\
+         connect_non_passive_type gts gtt /\
+         connect_non_passive_type_fields_flipped ft fs
+   | _, _ => False
+   end.
+*)
+
+Lemma set_find_sub : forall checkt nt nt0 n, ft_set_sub checkt nt n = Some nt0 -> ftype_equiv checkt nt0 -> ft_find_sub nt0 n = Some nt
+with set_find_sub_f : forall checkf nf nf0 n, ft_set_sub_f checkf nf n = Some nf0 -> fbtyp_equiv checkf nf0 -> ft_find_ff nf0 n = Some nf.
+Proof.
+  clear set_find_sub.
+  elim.
+  intro f.
+  intros nt nt0 n Hset Heq.
+  simpl in Heq.
+  simpl in Hset.
+  case Ha : (n == N0); rewrite Ha in Hset; try discriminate.
+  inversion Hset; clear Hset H0.
+  case Hnt0 : (nt0) => [f0||]; rewrite Hnt0 in Heq; try discriminate.
+  simpl; rewrite Ha; done.
+
+  intros f Hg fn. 
+  intros nt nt0 n Hset Heq.
+  simpl in Hset.
+  case Hset' : (ft_set_sub f nt n) => [natyp|]; rewrite Hset' in Hset; try discriminate.
+  inversion Hset; clear Hset.
+  simpl.
+  rewrite -H0 in Heq; simpl in Heq.
+  move /andP : Heq => [_ Heq].
+  apply Hg; try done.
+
+  intros f nt nt0 n Hset Heq.
+  simpl in Hset.
+  case Ha : (tmap_type_size_fields f <= n); rewrite Ha in Hset; try discriminate.
+  case Hset' : (ft_set_sub_f f nt n) => [newf|]; rewrite Hset' in Hset; try discriminate.
+  inversion Hset; clear Hset.
+  simpl.
+  assert (tmap_type_size_fields newf = tmap_type_size_fields f).
+  admit.
+  rewrite H; clear H; rewrite Ha.
+  rewrite -H0 in Heq; simpl in Heq.
+  apply set_find_sub_f with (checkf := f); try done.
+
+  (*clear set_find_sub_f.
+  intros checkf.
+  induction checkf.
+  intros nf a nf0 n Hset Heq.
+  simpl in Hset; discriminate.
+
+  intros nf a hf0 n Hset Heq.
+  simpl in Hset.
+  case Hf : f; rewrite Hf in Hset; try discriminate.
+  case Ha : (a.2 == (n + 1)%num); rewrite Ha in Hset.
+  inversion Hset; clear Hset.
+  simpl; rewrite Ha; done.
+  case Ha' : ((n + N.of_nat (num_ref f0))%num < a.2); rewrite Ha' in Hset.
+  case Hset' : (ft_set_sub_f a checkf nf (n + N.of_nat (num_ref f0))) => [newf|]; rewrite Hset' in Hset; try discriminate.
+  inversion Hset; clear Hset.
+  apply IHcheckf in Hset'.
+  simpl; rewrite Ha Ha'; done.
+  rewrite -H0 in Heq.
+  simpl in Heq; rewrite Hf in Heq.
+  move /andP : Heq => [_ Heq]; done. 
+
+  case Hset' : (ft_set_sub a f0 nf (n+1)) => [newt'|]; rewrite Hset' in Hset; try discriminate.
+  inversion Hset; clear Hset.
+  assert ((num_ref f0) = (num_ref newt')).
+  rewrite -H0 in Heq.
+  simpl in Heq.
+  rewrite Hf in Heq.
+  move /andP : Heq => [Heq _].
+  move /andP : Heq => [_ Heq].
+  apply num_ref_eq; done.
+  rewrite H in Ha'; clear H.
+  simpl; rewrite Ha Ha'.
+  apply set_find_sub with (checkt := f0); try done.
+  rewrite -H0 in Heq.
+  simpl in Heq; rewrite Hf in Heq.
+  move /andP : Heq => [Heq _].
+  move /andP : Heq => [_ Heq].
+  done.*)
+Admitted.
+
+Lemma ft_set_sub_eq : forall checkt nt' nt0 n init, ft_find_sub checkt n = Some init -> fgtyp_equiv init nt' -> ft_set_sub checkt nt' n = Some nt0 -> ftype_equiv checkt nt0
+with ft_set_sub_eq_f : forall checkf nf' nf0 n init, ft_find_ff checkf n = Some init -> fgtyp_equiv init nf' -> ft_set_sub_f checkf nf' n = Some nf0 -> fbtyp_equiv checkf nf0.
+Proof.
+(* in InferWidths.v *)
+Admitted.
+
+Lemma max_compatible : forall el tmap otype nt eftl, fil_ftlist [seq type_of_hfexpr e tmap | e <- el] = Some eftl -> max_ftlist eftl otype = Some nt -> forall expr exprtype, expr \in el -> type_of_hfexpr expr tmap = Some exprtype -> connect_type_compatible (Gtyp nt) exprtype.
+Proof.
+  elim.
+  intros.
+  rewrite in_nil in H1; discriminate.
+  intros hd tl H tmap init nt eftl Hl Hmax.
+  simpl in Hl. 
+  (*case Hhd : (type_of_e hd tmap) => [nht|]; rewrite Hhd in Hl; try discriminate.
+  case Hl' : (fil_ftlist [seq type_of_e e tmap | e <- tl]) => [tl'|]; rewrite Hl' in Hl; try discriminate.
+  inversion Hl; clear Hl.
+  rewrite -H1 in Hmax.
+  simpl in Hmax.
+  case Hmax' : (max_ftlist tl' init) => [nt'|]; rewrite Hmax' in Hmax; try discriminate.
+
+  intros expr exprtype Hin Hexpr.
+  rewrite in_cons in Hin.
+  case Heq : (expr == hd).
+  move /eqP : Heq => Heq.
+  rewrite Heq in Hexpr.
+  rewrite Hexpr in Hhd.
+  inversion Hhd; clear Hhd.
+  move : Hmax. (* infer_compatible *)
+  admit.
+  rewrite Heq in Hin; clear Heq. 
+  apply H with (tmap := tmap) (otype := init ) (nt := nt') (eftl := tl') (expr := expr) (exprtype := exprtype) in Hl'; try done.
+  apply connect_compatible_dlvr with (t1 := nt) (t2 := nt') (t3 := exprtype); try done.
+  move : Hmax.
+  apply infer_compatible.*)
+Admitted.
+
+Lemma inferwidths_a : forall a v expr_seq tmap tmap', InferWidth_fun v expr_seq tmap = Some tmap' -> 
+  if (a == v) then True 
+  else match CEP.find (fst a, N0) tmap, CEP.find (fst a, N0) tmap' with
+        | Some ft, Some ft' => ft_find_sub ft (snd a) = ft_find_sub ft' (snd a)
+        | _, _ => True
+        end.
+Proof.
+  (* 这个定理不对了
+  intros.
+  case Heq : (a == v); try done.
+  case Heq' : ((a.1 == v.1) && (a.2 != v.2)).
+  move /andP : Heq' => [H0 H1]; clear Heq.
+  move /eqP : H0 => H0.
+  rewrite H0. 
+  rewrite /InferWidth_fun in H.
+  case Hel : (fil_ftlist [seq type_of_e e tmap | e <- expr_seq]) => [eftl|]; rewrite Hel in H; try discriminate.
+  case Hfindv0 : (ft_find (v.1, 0%num) tmap) => [init|]; rewrite Hfindv0 in H; try discriminate.
+  case Hsub : (ft_find_sub v init 0) => [initt|]; rewrite Hsub in H; try discriminate.
+  case Hmax : (max_ftlist eftl initt) => [nt|]; rewrite Hmax in H; try discriminate.
+  case Hinfer : (InferWidth_ref v init nt) => [nt0|]; rewrite Hinfer in H; try discriminate.
+  inversion H; clear H.
+  rewrite ft_find_add.
+  rewrite /InferWidth_ref in Hinfer.
+  rewrite Hsub in Hinfer.
+  case Hinfer' : (infer_implicit initt nt) => [newt|]; rewrite Hinfer' in Hinfer; try discriminate.
+  (* forall a v, a.1 = v.1 -> a.2 != v.2 -> ft_set_sub v init newt 0 = Some nt0 -> ft_set_sub v init newt 0 = Some nt0. *)
+  admit. (* inferref只改了v位置上的，故find_sub a应该相等 *)
+  assert (a.1 != v.1).
+  admit. (* 由Heq Heq'推出a.1!=v.1 *)
+  rewrite /InferWidth_fun in H.
+  case Hel : (fil_ftlist [seq type_of_e e tmap | e <- expr_seq]) => [eftl|]; rewrite Hel in H; try discriminate.
+  case Hfindv0 : (ft_find (v.1, 0%num) tmap) => [init|]; rewrite Hfindv0 in H; try discriminate.
+  case Hsub : (ft_find_sub v init 0) => [initt|]; rewrite Hsub in H; try discriminate.
+  case Hmax : (max_ftlist eftl initt) => [nt|]; rewrite Hmax in H; try discriminate.
+  case Hinfer : (InferWidth_ref v init nt) => [nt0|]; rewrite Hinfer in H; try discriminate.
+  inversion H; clear H.
+  case Hfinda0 : (ft_find (a.1, 0%num) tmap) => [ft|]; try done.
+  (* find_add_not. forall a v nt tmap, ft_find a tmap = ft_find a (ft_add v nt tmap) *)
+  admit.  ft = ft' *)
+Admitted.
+
+Lemma inferwidths_ls : forall el a var2exprs tmap tmap' checkt checkt', InferWidths_fun el var2exprs tmap = Some tmap' -> 
+  ~(a \in el) -> CEP.find (fst a, N0) tmap' = Some checkt' -> CEP.find (fst a, N0) tmap = Some checkt -> ft_find_sub checkt (snd a) = ft_find_sub checkt' (snd a).
+Proof.
+ (* 这个定理不对了 *)
+  
+Admitted.
+
+Lemma InferWidth_fun_correct : forall pv el tmap newtm, InferWidth_fun pv el tmap = Some newtm -> forall expr, expr \in el -> 
+      match CEP.find (fst pv, N0) newtm with
+      | Some checkt => match ft_find_sub checkt pv.2, type_of_hfexpr expr newtm with
+                              | Some nt, Some te => ftype_equiv (Gtyp nt) te -> connect_type_compatible (Gtyp nt) te
+                              | _,_ => true
+                              end
+      | _ => true
+      end.
+Proof.
+  intros pv el tmap newtm Hinfer expr Hin.
+  rewrite /InferWidth_fun in Hinfer.
+  case Hel : (fil_ftlist [seq type_of_hfexpr e tmap | e <- el]) => [eftl|]; rewrite Hel in Hinfer; try discriminate.
+  case Hinit : (CEP.find (pv.1, 0%num) tmap) => [init|]; rewrite Hinit in Hinfer; try discriminate.
+  case Hinitt : (ft_find_sub init pv.2) => [initt|]; rewrite Hinitt in Hinfer; try discriminate.
+  case Hcheckt : (CEP.find (pv.1, 0%num) newtm) => [checkt|]; try done.
+  case Hnt : (ft_find_sub checkt pv.2) => [nt|]; try done.
+  case Hte : (type_of_hfexpr expr newtm) => [te|]; try done.
+  intro Heq.
+  case Himpli : (not_implicit initt); rewrite Himpli in Hinfer.
+  (* case 1 *)
+  rewrite /connect_type_compatible.
+  apply rwP with (P := ftype_equiv (Gtyp nt) te /\ check_connect_fgtyp_compatible (Gtyp nt) te (tmap_type_size (Gtyp nt))).
+  apply andP.
+  split; try done.
+  simpl.
+  case He : te => [gt||]; rewrite He in Heq; simpl in Heq; try discriminate.
+  simpl.
+  rewrite /connect_fgtyp_compatible.
+  inversion Hinfer; clear Hinfer.
+  rewrite H0 in Hinit; rewrite Hinit in Hcheckt; inversion Hcheckt; clear Hcheckt H0 Hinit.
+  rewrite H1 in Hinitt; rewrite Hinitt in Hnt; inversion Hnt; clear Hnt Hinitt H1.
+  rewrite H0 in Himpli; rewrite Himpli; done.
+  (* case2 *)
+  case Hmax : (max_ftlist eftl initt) => [tmax|]; rewrite Hmax in Hinfer; try discriminate.
+  case Hset : (ft_set_sub init tmax pv.2) => [nt0|]; rewrite Hset in Hinfer; try discriminate.
+  inversion Hinfer; clear Hinfer.
+  rewrite -H0 in Hte Hcheckt; clear H0.
+  rewrite HiFP.PCELemmas.OP.P.F.add_eq_o in Hcheckt.
+  inversion Hcheckt; clear Hcheckt.
+  rewrite -H0 in Hnt; clear H0.
+  apply set_find_sub in Hset; try done.
+  rewrite Hset in Hnt; clear Hset.
+  inversion Hnt; clear Hnt.
+  rewrite -H0; clear H0.
+  apply max_compatible with (el := el) (tmap := tmap) (otype := initt) (eftl := eftl) (expr := expr); try done.
+  admit. (* 由于不成环，不影响expr的type，由Hte *)
+  admit. (* ft_set 的性质，由Hset *)
+Admitted.
+
+Lemma InferWidths_fun_correct : forall (hfs : HiFP.hfstmt) (inferorder : seq ProdVarOrder.t) (var2exprs : var2exprsmap) (tmap newtm : CEP.t ftype),
+  InferWidths_fun inferorder var2exprs tmap = Some newtm -> match hfs with
+    | Sfcnct ref_tgt (Eref ref_src) => match base_ref ref_tgt newtm, base_ref ref_src newtm with
+                                      | Some (pv_tgt, t_tgt), Some (pv_src, t_src) => connect_non_passive_type t_tgt t_src
+                                      | _, _ => True
+                                      end 
+    | Sfcnct ref_tgt expr_src => match base_ref ref_tgt newtm, type_of_hfexpr expr_src newtm with
+                                      | Some tgt, Some t_expr => connect_type_compatible tgt.2 t_expr
+                                      | _, _ => True
+                                      end
+    | _ => True
+    end.
+Proof.
+  intros hfs inferorder var2exprs tmap newtm Hinfer.
+  case Hs : hfs => [||||||ref expr||]; try done.
+  case He : expr => [ct c| c e1 | u e1 | op e1 e2 | c e1 e2 | c e1 | ref0 ]. 
+  (* const *)
+  rewrite -He.
+  case Hbase : (base_ref ref newtm) => [tgt|]; try done.
+  case Hte : (type_of_hfexpr expr newtm) => [t_expr|] ; try done.
+  rewrite /connect_type_compatible.
+  apply rwP with (P := ftype_equiv tgt.2 t_expr /\
+    check_connect_fgtyp_compatible tgt.2 t_expr (tmap_type_size tgt.2)).
+  apply andP.
+  split. 
+  admit. (* 对connection语句的要求 *)
+
+  assert (forall ft te, (forall n gt gte, n < tmap_type_size ft -> ft_find_sub ft (N.of_nat n) = Some gt -> ft_find_sub te (N.of_nat n) = Some gte ->
+        connect_fgtyp_compatible gt gte) ->
+    check_connect_fgtyp_compatible ft te (tmap_type_size ft)).
+  admit.
+
+  apply H; clear H.
+  intros n gt gte Hn Hlhs Hrhs.
+  assert ((tgt.1.1, N.add tgt.1.2 (N.of_nat n)) \in inferorder).
+  admit. (* inferorder 的正确性，是展开时的标号 *)
+  assert (exists order1 order2, inferorder = order1 ++ ((tgt.1.1, N.add tgt.1.2 (N.of_nat n)) :: order2) /\ ~ (tgt.1.1, N.add tgt.1.2 (N.of_nat n)) \in order1 /\ ~ (tgt.1.1, N.add tgt.1.2 (N.of_nat n)) \in order2).
+  admit. (* 由H推出 *)
+  clear H.
+  move : H0 => [order1 [order2 [H [Horder1 Horder2]]]].
+  rewrite H in Hinfer; rewrite /InferWidths_fun in Hinfer.
+  case Hinfer1 : (InferWidths_fun order1 var2exprs tmap) => [tmap'|].
+  assert (Hinfer2 : InferWidths_fun ((tgt.1.1, N.add tgt.1.2 (N.of_nat n)) :: order2) var2exprs tmap' = Some newtm).
+  admit. (* 由 Hinfer Hinfer1 *)
+  clear Hinfer.
+  simpl in Hinfer2.
+  case Hel : (module_graph_vertex_set_p.find (tgt.1.1, N.add tgt.1.2 (N.of_nat n)) var2exprs) => [el|]; rewrite Hel in Hinfer2; try done.
+  case Hinfer : (InferWidth_fun (tgt.1.1, N.add tgt.1.2 (N.of_nat n)) el tmap') => [newtm'|]; rewrite Hinfer in Hinfer2; try discriminate.
+
+  assert (forall expr rhs_expr_ls t_expr newtm, type_of_hfexpr expr newtm = Some t_expr -> split_expr_connect expr t_expr = Some rhs_expr_ls ->  (* 这里可以加bool list用来判断flip *)
+            forall n, n < length rhs_expr_ls -> match List.nth_error rhs_expr_ls n, ft_find_sub t_expr (N.of_nat n) with
+                                    | Some texpr, Some gt => type_of_hfexpr texpr newtm = Some (Gtyp gt)
+                                    | _, _ => true
+                                    end). 
+  admit. (* split和typeofexpr的性质 *)
+
+  case Hsplit : (split_expr_connect expr t_expr) => [rhs_expr_ls|].
+  apply H0 with (expr := expr) (rhs_expr_ls := rhs_expr_ls) (t_expr := t_expr) (newtm := newtm) (n := n) in Hsplit; try done; clear H0.
+  case Htexpr : (nth_error rhs_expr_ls n) => [texpr|]; rewrite Htexpr in Hsplit.
+  rewrite Hrhs in Hsplit.
+
+  apply InferWidth_fun_correct with (pv := (tgt.1.1, N.add tgt.1.2 (N.of_nat n))) (el := el) (tmap := tmap') (newtm := newtm') (expr := texpr) in Hinfer.
+  simpl in Hinfer.
+  case Htgt0 : (CEP.find (tgt.1.1, 0%num) newtm') => [checkt'|]; rewrite Htgt0 in Hinfer.
+  case Hsub0 : (ft_find_sub checkt' (tgt.1.2 + N.of_nat n)) => [nt|]; rewrite Hsub0 in Hinfer.
+  case Htgt : (CEP.find (tgt.1.1, 0%num) newtm) => [checkt|].
+  apply inferwidths_ls with (var2exprs := var2exprs) (tmap := newtm') (tmap' := newtm) (checkt := checkt') (checkt' := checkt) in Horder2; try done.
+  rewrite Hsub0 in Horder2; clear Hsub0.
+  simpl in Horder2.
+
+  assert (forall ref n pv ft tmap, base_ref ref tmap = Some (pv, ft) -> CEP.find (tgt.1.1, 0%num) tmap = Some checkt -> ft_find_sub checkt (tgt.1.2 + N.of_nat n) = ft_find_sub tgt.2 (N.of_nat n)).
+  admit. (* 两种返回ftype函数的关系和正确性 *)
+
+  specialize H0 with (ref := ref) (n := n) (pv := tgt.1) (ft := tgt.2) (tmap := newtm).
+  apply H0 in Htgt; clear H0; try done.
+  rewrite Htgt in Horder2; clear Htgt.
+  rewrite Hlhs in Horder2; clear Hlhs.
+  inversion Horder2; clear Horder2.
+
+  case Hte' : (type_of_hfexpr texpr newtm') => [te|]; rewrite Hte' in Hinfer.
+  assert (type_of_hfexpr texpr newtm = Some te).
+  admit. (* 由于拓扑排序，texpr不受order2中的位宽更新影响。由Hte' Hinfer2 *)
+  clear Hte'.
+  rewrite H0 in Hsplit.
+  inversion Hsplit; clear Hsplit.
+  rewrite H3 H1 in Hinfer.
+  rewrite /connect_type_compatible in Hinfer.
+  assert (fgtyp_equiv gt gte).
+  admit. (* 从某个地方来的连接合法的前提 *)
+  apply Hinfer in H2; clear Hinfer.
+  move /andP : H2 => [_ Hinfer].
+  simpl in Hinfer. 
+  move /andP : Hinfer => [Hinfer _]; done.
+
+  admit. (* type_of_hfexpr 不为None，由Htgt0 *)
+  admit. (* eta_expand这是啥，有Hbase *)
+  admit. (* 由Htgt0不为None *)
+  admit. (* 由 n < tmap_type_size tgt.2 知Hsub0不为None *)
+  admit. (* 被连接的应该已被声明，find不为None *)
+  admit. (* var2exprs应当满足的性质，由add_expr_connect *)
+  admit. (* n 不超过 rhs_expe_ls 的长度，不为None *)
+  assert (length rhs_expr_ls = tmap_type_size tgt.2).
+  admit. (* 由split_expr_connect的性质 *)
+  rewrite H0; clear H0; done.
+  admit. (* expr应该与t_expr匹配，不会出错 *)
+  admit. (* 若infer order1有错误，则infer没有结果 *)
+
+  (* 所有passive的expr都一样 *)
+  admit.
+  admit.
+  admit.
+  admit.
+  admit.
+
+  (* ref non_passive *)
+  case Htgt : (base_ref ref newtm) => [[v_tgt t_tgt]|]; try done.
+  case Hsrc : (base_ref ref0 newtm) => [[v_src t_src]|]; try done.
+  rewrite /connect_non_passive_type.
+  apply rwP with (P := ftype_equiv t_tgt t_src /\ check_connect_non_passive_fgtyp t_tgt t_src (tmap_type_size t_tgt)).
+  apply andP.
+  split. 
+  admit. (* 对connection语句的要求 *)
+
+  assert (forall ft te, (forall n gt gte, n < tmap_type_size ft -> ft_find_sub ft (N.of_nat n) = Some gt -> ft_find_sub te (N.of_nat n) = Some gte ->
+        match ft_check_flip ft (N.of_nat n) false with
+        | Some false => connect_fgtyp_compatible gt gte
+        | Some true => connect_fgtyp_compatible gte gt
+        | None => false
+        end) ->
+        check_connect_non_passive_fgtyp ft te (tmap_type_size ft)).
+  admit.
+
+  apply H; clear H.
+  intros n gt gte Hn Hlhs Hrhs.
+
+  (* stop here, 在拆开infer之前，应该确定lhs or rhs的pv in inferorder *)
+  (* TBD!! *)
+  
+  assert ((v_tgt.1, N.add v_tgt.2 (N.of_nat n)) \in inferorder).
+  admit. (* inferorder 的正确性，是展开时的标号 *)
+  assert (exists order1 order2, inferorder = order1 ++ ((v_tgt.1, N.add v_tgt.2 (N.of_nat n)) :: order2) /\ ~ (v_tgt.1, N.add v_tgt.2 (N.of_nat n)) \in order1 /\ ~ (v_tgt.1, N.add v_tgt.2 (N.of_nat n)) \in order2).
+  admit. (* 由H推出 *)
+  clear H.
+  move : H0 => [order1 [order2 [H [Horder1 Horder2]]]].
+  rewrite H in Hinfer; rewrite /InferWidths_fun in Hinfer.
+  case Hinfer1 : (InferWidths_fun order1 var2exprs tmap) => [tmap'|].
+  assert (Hinfer2 : InferWidths_fun ((v_tgt.1, N.add v_tgt.2 (N.of_nat n)) :: order2) var2exprs tmap' = Some newtm).
+  admit. (* 由 Hinfer Hinfer1 *)
+  clear Hinfer.
+  simpl in Hinfer2.
+  case Hel : (module_graph_vertex_set_p.find (v_tgt.1, N.add v_tgt.2 (N.of_nat n)) var2exprs) => [el|]; rewrite Hel in Hinfer2; try done.
+  case Hinfer : (InferWidth_fun (v_tgt.1, N.add v_tgt.2 (N.of_nat n)) el tmap') => [newtm'|]; rewrite Hinfer in Hinfer2; try discriminate.
+
+  assert (forall ref_tgt ref_src t_tgt t_src v_tgt v_src tmap, base_ref ref_tgt tmap = Some (v_tgt, t_tgt) -> base_ref ref_src tmap = Some (v_src, t_src) ->
+              match split_expr_non_passive ref_tgt t_tgt false, split_expr_non_passive ref_src t_src false with
+              | Some lhsl, Some rhsl => (forall n, n < length lhsl -> match List.nth_error lhsl n, List.nth_error rhsl n with
+                                        | Some (_, false), Some (ref2, false) => match module_graph_vertex_set_p.find (v_tgt.1, N.add v_tgt.2 (N.of_nat n)) var2exprs with
+                                                          | Some el => (Eref ref2) \in el
+                                                          | None => false
+                                                          end
+                                        | Some (ref1, true), Some (_, true) => match module_graph_vertex_set_p.find (v_src.1, N.add v_src.2 (N.of_nat n)) var2exprs with
+                                                          | Some el => (Eref ref1) \in el
+                                                          | None => false
+                                                          end
+                                        | _,_ => false
+                                        end)
+              | _, _ => false
+              end). 
+  admit. (* split和存var2exprs的性质 *)
+  apply H0 with (ref_tgt := ref) (t_tgt := t_tgt) (v_tgt := v_tgt) (ref_src := ref0) (t_src := t_src) (v_src := v_src) in Htgt; try done; clear H0.
+  case Hsplit_lhs : (split_expr_non_passive ref t_tgt false) => [lhsl|]; rewrite Hsplit_lhs in Htgt.
+  case Hsplit_rhs : (split_expr_non_passive ref0 t_src false) => [rhsl|]; rewrite Hsplit_rhs in Htgt.
+  assert (length lhsl = tmap_type_size t_tgt).
+  admit.
+  rewrite H0 in Htgt; clear H0.
+  apply Htgt in Hn; clear Htgt.
+  
+  case Hlhsl : (nth_error lhsl n) => [[ref1 b1]|]; rewrite Hlhsl in Hn.
+  case Hrhsl : (nth_error rhsl n) => [[ref2 b2]|]; rewrite Hrhsl in Hn.
+  case Hcheckfl : (ft_check_flip t_tgt (N.of_nat n) false) => [b1'|].
+  assert (b1 = b1').
+  admit. (* 两种不同的算flip方法应当结果相同 *)
+  assert (b1 = b2). (* tgt和src类型相同 *)
+  admit.
+
+  case Hb : b1; rewrite Hb in H0 Hn H1; rewrite -H0; rewrite -H1 in Hn.
+  (* case1 : flip field *)
+  apply InferWidth_fun_correct with (pv := (v_src.1, (v_src.2 + N.of_nat n)%num)) (el := el) (tmap := tmap') (newtm := newtm') (expr := (Eref ref1)) in Hinfer.
+  simpl in Hinfer.
+  case Htgt0 : (CEP.find (tgt.1.1, 0%num) newtm') => [checkt'|]; rewrite Htgt0 in Hinfer.
+  case Hsub0 : (ft_find_sub checkt' (tgt.1.2 + N.of_nat n)) => [nt|]; rewrite Hsub0 in Hinfer.
+  case Htgt : (CEP.find (tgt.1.1, 0%num) newtm) => [checkt|].
+  apply inferwidths_ls with (var2exprs := var2exprs) (tmap := newtm') (tmap' := newtm) (checkt := checkt') (checkt' := checkt) in Horder2; try done.
+  rewrite Hsub0 in Horder2; clear Hsub0.
+  simpl in Horder2.
+
+  assert (forall ref n pv ft tmap, base_ref ref tmap = Some (pv, ft) -> CEP.find (tgt.1.1, 0%num) tmap = Some checkt -> ft_find_sub checkt (tgt.1.2 + N.of_nat n) = ft_find_sub tgt.2 (N.of_nat n)).
+  admit. (* 两种返回ftype函数的关系和正确性 *)
+
+Admitted.
+
+Definition InferWidths_m F :=
+  match InferWidths_stage1 F with
+  | Some newtm => InferWidths_stage2 F newtm 
+  | None => None
+  end.
+
+Lemma InferWidths_correct : forall (F : HiFP.hfmodule) (vm' : module_graph_vertex_set_p.env) (ct : module_graph_connection_trees_p.env),
+  match InferWidths_m F with
+  | Some F' => Sem F' vm' ct -> Sem F (make_vm_implicit F vm') ct
+  | _ => True
+  end.
+Proof.
+  
+Admitted.
+
+Fixpoint fillft_vm (n : nat) (ft : ftype) (pv : ProdVarOrder.t) (vmap : module_graph_vertex_set_p.env) : option ftype :=
+   match n with
+   | 0 => Some ft
+   | S m => match module_graph_vertex_set_p.find (fst pv, (N.add (snd pv) (N.of_nat m))) vmap with
+            | Some nt => match List.hd_error (input_connectors nt) with
+                        | Some gt => match ft_set_sub (fst pv, (N.add (snd pv) (N.of_nat m))) ft (Gtyp gt) (snd pv) with
+                                   | Some nft => fillft_vm m nft pv vmap
+                                   | None => None
+                                   end
+                       | None => None
+                       end
+           | None => None
+           end
+   end.
+
+Fixpoint type_of_hfexpr_vm (vmap : module_graph_vertex_set_p.env) (e : HiFP.hfexpr) (tmap : CEP.t ftype) : option ftype :=
+   match e with
+   | Econst t bs => match t with
+                    | Fuint_implicit w => Some (Gtyp (Fuint (size bs)))
+                    | Fsint_implicit w => Some (Gtyp (Fsint (size bs)))
+                    | t => Some (Gtyp t)
+                    end
+   | Eref r => match base_ref r tmap with
+              | Some (pv, checkt) => fillft_vm (tmap_type_size checkt) checkt pv vmap
+              | None => None
+              end
+   | Ecast AsUInt e1 => match type_of_hfexpr_vm vmap e1 tmap with
+                         | Some (Gtyp (Fsint w))
+                         | Some (Gtyp (Fuint w)) => Some (Gtyp (Fuint w))
+                         | Some (Gtyp Fclock)
+                         | Some (Gtyp Freset)
+                         | Some (Gtyp Fasyncreset) => Some (Gtyp (Fuint 1))
+                         | _ => None
+                         end
+   | Ecast AsSInt e1 => match type_of_hfexpr_vm vmap e1 tmap with
+                         | Some (Gtyp (Fsint w))
+                         | Some (Gtyp (Fuint w)) => Some (Gtyp (Fsint w))
+                         | Some (Gtyp Fclock)
+                         | Some (Gtyp Freset)
+                         | Some (Gtyp Fasyncreset) => Some (Gtyp (Fsint 1))
+                         | _ => None
+                         end
+   | Ecast AsClock e1 => match type_of_hfexpr_vm vmap e1 tmap with
+                         | Some (Gtyp _) => Some (Gtyp Fclock)
+                         | _ => None
+                         end
+   | Ecast AsAsync e1 => match type_of_hfexpr_vm vmap e1 tmap with
+                         | Some (Gtyp _) => Some (Gtyp Fasyncreset)
+                         | _ => None
+                         end
+   | Eprim_unop (Upad n) e1 => match type_of_hfexpr_vm vmap e1 tmap with
+                                | Some (Gtyp (Fsint w)) => Some (Gtyp (Fsint (maxn w n)))
+                                | Some (Gtyp (Fuint w)) => Some (Gtyp (Fuint (maxn w n)))
+                                | _ => None
+                                end
+   | Eprim_unop (Ushl n) e1 => match type_of_hfexpr_vm vmap e1 tmap with
+                                | Some (Gtyp (Fsint w)) => Some (Gtyp (Fsint (w + n)))
+                                | Some (Gtyp (Fuint w)) => Some (Gtyp (Fuint (w + n)))
+                                | _ => None
+                                end
+   | Eprim_unop (Ushr n) e1 => match type_of_hfexpr_vm vmap e1 tmap with
+                                | Some (Gtyp (Fsint w)) => Some (Gtyp (Fsint (maxn (w - n) 1)))
+                                | Some (Gtyp (Fuint w)) => Some (Gtyp (Fuint (maxn (w - n) 1)))
+                                | _ => None
+                                end
+   | Eprim_unop Ucvt e1 => match type_of_hfexpr_vm vmap e1 tmap with
+                            | Some (Gtyp (Fsint w)) => Some (Gtyp (Fsint w))
+                            | Some (Gtyp (Fuint w)) => Some (Gtyp (Fsint (w + 1)))
+                            | _ => None
+                            end
+   | Eprim_unop Uneg e1 => match type_of_hfexpr_vm vmap e1 tmap with
+                            | Some (Gtyp (Fsint w))
+                            | Some (Gtyp (Fuint w)) => Some (Gtyp (Fsint (w + 1)))
+                            | _ => None
+                            end
+   | Eprim_unop Unot e1 => match type_of_hfexpr_vm vmap e1 tmap with
+                            | Some (Gtyp (Fsint w))
+                            | Some (Gtyp (Fuint w)) => Some (Gtyp (Fuint w))
+                            | _ => None
+                            end
+   | Eprim_unop (Uextr n1 n2) e1 => match type_of_hfexpr_vm vmap e1 tmap with
+                                     | Some (Gtyp (Fsint w))
+                                     | Some (Gtyp (Fuint w)) =>
+                                          if (n2 <= n1) && (n1 < w) then Some (Gtyp (Fuint (n1 - n2 + 1)))
+                                                                    else None
+                                     | _ => None
+                                     end
+   | Eprim_unop (Uhead n) e1 => match type_of_hfexpr_vm vmap e1 tmap with
+                                 | Some (Gtyp (Fsint w))
+                                 | Some (Gtyp (Fuint w)) =>
+                                      if n <= w then Some (Gtyp (Fuint n))
+                                                else None
+                                 | _ => None
+                                 end
+   | Eprim_unop (Utail n) e1 => match type_of_hfexpr_vm vmap e1 tmap with
+                                 | Some (Gtyp (Fsint w))
+                                 | Some (Gtyp (Fuint w)) =>
+                                      if n <= w then Some (Gtyp (Fuint (w - n)))
+                                                else None
+                                 | _ => None
+                                 end
+   | Eprim_unop _ e1 => match type_of_hfexpr_vm vmap e1 tmap with
+                         | Some (Gtyp (Fsint _))
+                         | Some (Gtyp (Fuint _)) => Some (Gtyp (Fuint 1))
+                         | _ => None
+                         end
+   | Eprim_binop (Bcomp _) e1 e2 => match type_of_hfexpr_vm vmap e1 tmap, type_of_hfexpr_vm vmap e2 tmap with
+                                     | Some (Gtyp (Fsint _)), Some (Gtyp (Fsint _))
+                                     | Some (Gtyp (Fuint _)), Some (Gtyp (Fuint _)) => Some (Gtyp (Fuint 1))
+                                     | _, _ => None
+                                     end
+   | Eprim_binop Badd e1 e2
+   | Eprim_binop Bsub e1 e2 => match type_of_hfexpr_vm vmap e1 tmap, type_of_hfexpr_vm vmap e2 tmap with
+                                | Some (Gtyp (Fuint w1)), Some (Gtyp (Fuint w2)) => Some (Gtyp (Fuint (maxn w1 w2 + 1)))
+                                | Some (Gtyp (Fsint w1)), Some (Gtyp (Fsint w2)) => Some (Gtyp (Fsint (maxn w1 w2 + 1)))
+                                | _, _ => None
+                                end
+   | Eprim_binop Bmul e1 e2 => match type_of_hfexpr_vm vmap e1 tmap, type_of_hfexpr_vm vmap e2 tmap with
+                                | Some (Gtyp (Fuint w1)), Some (Gtyp (Fuint w2)) => Some (Gtyp (Fuint (w1 + w2)))
+                                | Some (Gtyp (Fsint w1)), Some (Gtyp (Fsint w2)) => Some (Gtyp (Fsint (w1 + w2)))
+                                | _, _ => None
+                                end
+   | Eprim_binop Bdiv e1 e2  => match type_of_hfexpr_vm vmap e1 tmap, type_of_hfexpr_vm vmap e2 tmap with
+                                 | Some (Gtyp (Fuint w1)), Some (Gtyp (Fuint w2)) => Some (Gtyp (Fuint w1))
+                                 | Some (Gtyp (Fsint w1)), Some (Gtyp (Fsint w2)) => Some (Gtyp (Fsint (w1 + 1)))
+                                 | _, _ => None
+                                 end
+   | Eprim_binop Brem e1 e2 => match type_of_hfexpr_vm vmap e1 tmap, type_of_hfexpr_vm vmap e2 tmap with
+                                 | Some (Gtyp (Fuint w1)), Some (Gtyp (Fuint w2)) => Some (Gtyp (Fuint (minn w1 w2)))
+                                 | Some (Gtyp (Fsint w1)), Some (Gtyp (Fsint w2)) => Some (Gtyp (Fsint (minn w1 w2)))
+                                 | _, _ => None
+                                 end
+   | Eprim_binop Bdshl e1 e2 => match type_of_hfexpr_vm vmap e1 tmap, type_of_hfexpr_vm vmap e2 tmap with
+                                 | Some (Gtyp (Fuint w1)), Some (Gtyp (Fuint w2)) => Some (Gtyp (Fuint (w1 + 2 ^ w2 - 1)))
+                                 | Some (Gtyp (Fsint w1)), Some (Gtyp (Fuint w2)) => Some (Gtyp (Fsint (w1 + 2 ^ w2 - 1)))
+                                 | _, _ => None
+                                 end
+   | Eprim_binop Bdshr e1 e2 => match type_of_hfexpr_vm vmap e1 tmap, type_of_hfexpr_vm vmap e2 tmap with
+                                 | Some (Gtyp (Fuint w1)), Some (Gtyp (Fuint w2)) => Some (Gtyp (Fuint w1))
+                                 | Some (Gtyp (Fsint w1)), Some (Gtyp (Fuint w2)) => Some (Gtyp (Fsint w1))
+                                 | _, _ => None
+                                 end
+   | Eprim_binop Bcat e1 e2 => match type_of_hfexpr_vm vmap e1 tmap, type_of_hfexpr_vm vmap e2 tmap with
+                                | Some (Gtyp (Fuint w1)), Some (Gtyp (Fuint w2))
+                                | Some (Gtyp (Fsint w1)), Some (Gtyp (Fsint w2)) => Some (Gtyp (Fuint (w1 + w2)))
+                                | _, _ => None
+                                end
+   | Eprim_binop Band e1 e2
+   | Eprim_binop Bor e1 e2
+   | Eprim_binop Bxor e1 e2 => match type_of_hfexpr_vm vmap e1 tmap, type_of_hfexpr_vm vmap e2 tmap with
+                                | Some (Gtyp (Fuint w1)), Some (Gtyp (Fuint w2))
+                                | Some (Gtyp (Fsint w1)), Some (Gtyp (Fsint w2)) => Some (Gtyp (Fuint (maxn w1 w2)))
+                                | _, _ => None
+                                end
+   | Emux c e1 e2 => match type_of_hfexpr_vm vmap c tmap, type_of_hfexpr_vm vmap e1 tmap, type_of_hfexpr_vm vmap e2 tmap with
+                      | Some (Gtyp (Fuint 1)), Some t1, Some t2 => mux_types t1 t2
+                      | _, _, _ => None
+                      end
+   | Evalidif c e1 => match type_of_hfexpr_vm vmap c tmap with
+                      | Some (Gtyp (Fuint 1)) => type_of_hfexpr_vm vmap e1 tmap
+                      | _ => None
+                      end
+   | _ => None (* Some (Gtyp (Fuint 0)) *)
+   end.
+
+Lemma InferWidths_fun_correct' F : forall vmap inferorder var2exprs tmap ct, Sem F vmap ct -> 
+  forall v, v \in inferorder -> 
+        match module_graph_vertex_set_p.find v vmap, module_graph_vertex_set_p.find v var2exprs, CEP.find (fst v, N0) tmap with
+        | Some nt, Some el, Some init => match List.hd_error (input_connectors nt), fil_ftlist (map (fun e => type_of_hfexpr_vm vmap e tmap) el), ft_find_sub v init N0 with
+                    | Some gt, Some eftl, Some (Gtyp initt) => match max_ftlist eftl initt with
+                                                        | Some nt => sizeof_fgtyp gt >= sizeof_fgtyp nt
+                                                        | _ => true
+                                                        end
+                    | _,_,_ => true
+                    end
+        | _,_,_ => true
+        end.
+Proof.
+  
+Qed.
